# imports: https://ontology.unifiedcyberontology.org/uco/role/1.1.0

@prefix core: <https://ontology.unifiedcyberontology.org/uco/core/> .
@prefix owl: <http://www.w3.org/2002/07/owl#> .
@prefix rdf: <http://www.w3.org/1999/02/22-rdf-syntax-ns#> .
@prefix rdfs: <http://www.w3.org/2000/01/rdf-schema#> .
@prefix role: <https://ontology.unifiedcyberontology.org/uco/role/> .
@prefix scope-role: <https://ontology.scopeontology.org/scope/role/> .
@prefix sh: <http://www.w3.org/ns/shacl#> .
@prefix xsd: <http://www.w3.org/2001/XMLSchema#> .

<https://ontology.scopeontology.org/scope/role>
	a owl:Ontology ;
	rdfs:label "scope-role"@en ;
	rdfs:comment "This ontology defines roles present in a Smart City Infrastructure (SCI) cybercrime investigation, identification of digital forensic opportunities and threat modeling."@en ;
	owl:imports role:1.1.0 ;
	owl:versionIRI scope-role:0.1.0 ;
	.

scope-role:Adversary
	a
		owl:Class ,
		sh:NodeShape
		;
	rdfs:subClassOf role:MaliciousRole ;
	rdfs:label "Adversary"@en ;
	rdfs:comment "An individual that seeks to disrupt or cause negative impacts to SCI."@en ;
	sh:targetClass role:Adversary ;
	.

scope-role:GovernmentDigitalForensicInvestigator
	a
		owl:Class ,
		sh:NodeShape
		;
	rdfs:subClassOf role:BenevolentRole ;
	rdfs:label "GovernmentDigitalForensicInvestigator"@en ;
	rdfs:comment "An individual tasked to investigate cybercrime and cyber attacks and working for a government agency."@en ;
	sh:targetClass role:GovernmentDigitalForensicInvestigator ;
	.

scope-role:LawEnforcementOfficer
	a
		owl:Class ,
		sh:NodeShape
		;
	rdfs:subClassOf role:BenevolentRole ;
	rdfs:label "LawEnforcementOfficer"@en ;
	rdfs:comment "An individual tasked to investigate cybercrime and cyber attacks and working for a law enforcement agency (LEA)."@en ;
	sh:targetClass role:LawEnforcementOfficer ;
	.

scope-role:PrivateDigitalForensicInvestigator
	a
		owl:Class ,
		sh:NodeShape
		;
	rdfs:subClassOf role:BenevolentRole ;
	rdfs:label "DigitalForensicInvestigator"@en ;
	rdfs:comment "An individual tasked to investigate cybercrime and cyber attacks and working for consulting or private companies."@en ;
	sh:targetClass role:DigitalForensicInvestigator ;
	.

scope-role:SmartCityInfrastructureOperator
	a
		owl:Class ,
		sh:NodeShape
		;
	rdfs:subClassOf role:NeutralRole ;
	rdfs:label "SmartCityInfrastructureOperator"@en ;
	rdfs:comment "An individual tasked to operate SCI systems."@en ;
	sh:targetClass role:SmartCityInfrastructureOperator ;
	.

scope-role:SmartCityInfrastructureUser
	a
		owl:Class ,
		sh:NodeShape
		;
	rdfs:subClassOf role:NeutralRole ;
	rdfs:label "SmartCityInfrastructureUser"@en ;
	rdfs:comment "An individual that uses the SCI systems."@en ;
	sh:targetClass role:SmartCityInfrastructureUser ;
	.

