# imports: https://ontology.unifiedcyberontology.org/uco/core/1.1.0
# imports: https://ontology.unifiedcyberontology.org/uco/observable/1.1.0

@prefix core: <https://ontology.unifiedcyberontology.org/uco/core/> .
@prefix evidence: <https://ontology.scopeontology.org/scope/evidence/> .
@prefix observable: <https://ontology.unifiedcyberontology.org/uco/observable/> .
@prefix owl: <http://www.w3.org/2002/07/owl#> .
@prefix rdf: <http://www.w3.org/1999/02/22-rdf-syntax-ns#> .
@prefix rdfs: <http://www.w3.org/2000/01/rdf-schema#> .
@prefix sh: <http://www.w3.org/ns/shacl#> .
@prefix xsd: <http://www.w3.org/2001/XMLSchema#> .

<https://ontology.scopeontology.org/scope/evidence>
	a owl:Ontology ;
	rdfs:label "scope-evidence"@en ;
	rdfs:comment "This ontology follows the definition of Smart City Infrastructure (SCI) defined in this paper (https://doi.org/10.48550/arxiv.2210.14692). Additional observables (evidence in our case) that is present in SCI and Internet-of-Things (IoT) devices that are currently not listed in uco-observable are placed here. This ontology also provides an opportunity for SCI related evidence to be listed here in future when SCI becomes more mature. Finally, this ontology can also contain legal terms that are used in courts."@en ;
	owl:imports
		core:1.1.0 ,
		observable:1.1.0
		;
	owl:versionIRI evidence:0.1.0 ;
	.

evidence:CitizenServiceSystemEvidence
	a
		owl:Class ,
		sh:NodeShape
		;
	rdfs:subClassOf evidence:SmartCityEvidence ;
	rdfs:label "CitizenServiceSystemEvidence"@en ;
	rdfs:comment "Evidence originating from Citizen Service System (systems that oversee data indicators from economy, education, finance, governance and housing)."@en ;
	sh:targetClass evidence:CitizenServiceSystemEvidence ;
	.

evidence:EssentialServiceSystemEvidence
	a
		owl:Class ,
		sh:NodeShape
		;
	rdfs:subClassOf evidence:SmartCityEvidence ;
	rdfs:label "EssentialServiceSystemEvidence"@en ;
	rdfs:comment "Evidence originating from Essential Service System (systems that oversee data indicators from health, safety, solid waste, telecommunication, transportation and wastewater)."@en ;
	sh:targetClass evidence:EssentialServiceSystemEvidence ;
	.

evidence:Evidence
	a
		owl:Class ,
		sh:NodeShape
		;
	rdfs:subClassOf observable:ObservableObject ;
	rdfs:label "Evidence"@en ;
	rdfs:comment "Information drawn from objects such as personal testimony, a document, digital or physical objects that is used to establish facts in a legal investigation or admissible as testimony in a court of law."@en ;
	sh:targetClass evidence:Evidence ;
	.

evidence:Firmware
	a
		owl:Class ,
		sh:NodeShape
		;
	rdfs:subClassOf evidence:Evidence ;
	rdfs:label "Firmware"@en ;
	rdfs:comment "Firmware images are purpose-built software operating systems that give embedded devices their functionality. This could be placed inside uco-observable in future."@en ;
	sh:targetClass evidence:Evidence ;
	.

evidence:FirmwareFacet
	a
		owl:Class ,
		sh:NodeShape
		;
	rdfs:subClassOf core:Facet ;
	rdfs:label "FirmwareFacet"@en ;
	rdfs:comment "A firmware facet is a grouping of characteristics unique to the software that manages embedded device hardware, software resources, and functionality. This could be placed inside uco-observable in future. "@en ;
	sh:targetClass evidence:FirmwareFacet ;
	.

evidence:LivelihoodSupportSystemEvidence
	a
		owl:Class ,
		sh:NodeShape
		;
	rdfs:subClassOf evidence:SmartCityEvidence ;
	rdfs:label "LivelihoodSupportSystemEvidence"@en ;
	rdfs:comment "Evidence originating from Livelihood Support System (systems that oversee data indicators from environment and climate change, population and social conditions, recreation, sport and culture, urban/local agriculture and food security and urban planning)."@en ;
	sh:targetClass evidence:LivelihoodSupportSystemEvidence ;
	.

evidence:ResourceSystemEvidence
	a
		owl:Class ,
		sh:NodeShape
		;
	rdfs:subClassOf evidence:SmartCityEvidence ;
	rdfs:label "ResourceSystemEvidence"@en ;
	rdfs:comment "Evidence originating from Livelihood Support System (systems that oversee data indicators from energy and water)."@en ;
	sh:targetClass evidence:ResourceSystemEvidence ;
	.

evidence:SmartCityEvidence
	a
		owl:Class ,
		sh:NodeShape
		;
	rdfs:subClassOf evidence:Evidence ;
	rdfs:label "SmartCityEvidence"@en ;
	rdfs:comment "Evidence related to Smart City Infrastructure. "@en ;
	sh:targetClass evidence:SmartCityEvidence ;
	.

evidence:SmartCitySystemEvidence
	a
		owl:Class ,
		sh:NodeShape
		;
	rdfs:subClassOf evidence:SmartCityEvidence ;
	rdfs:label "SmartCitySystemEvidence"@en ;
	rdfs:comment "Evidence originating from Smart City System (systems that oversee Citizen Service System, Essential Service System, Livelihood Support System and Resource System)."@en ;
	sh:targetClass evidence:SmartCitySystemEvidence;
	.

evidence:Testimony
	a
		owl:Class ,
		sh:NodeShape
		;
	rdfs:subClassOf evidence:Evidence ;
	rdfs:label "Testimony"@en ;
	rdfs:comment "A formal written or spoken statement that is given in a court of law. "@en ;
	sh:property
		[
			sh:datatype xsd:boolean ;
			sh:maxCount "1"^^xsd:integer ;
			sh:nodeKind sh:Literal ;
			sh:path evidence:evidenceAdmissible ;
		] ,
		[
			sh:datatype xsd:dateTime ;
			sh:maxCount "1"^^xsd:integer ;
			sh:nodeKind sh:Literal ;
			sh:path evidence:testimonyDate ;
		] ,
		[
			sh:datatype xsd:string ;
			sh:maxCount "1"^^xsd:integer ;
			sh:nodeKind sh:Literal ;
			sh:path evidence:testimonyOrigin ;
		]
		;
	sh:targetClass evidence:Testimony ;
	.

evidence:evidenceAdmissible
	a owl:DatatypeProperty ;
	rdfs:label "evidenceAdmissible"@en ;
	rdfs:comment "Specifies whether the evidence is admissible in a court of law."@en ;
	rdfs:range xsd:boolean ;
	.

evidence:firmwareCompileDate
	a owl:DatatypeProperty ;
	rdfs:label "firmwareCompileDate"@en ;
	rdfs:comment "The compilation date for the build of a firmware. This could be placed inside uco-observable in future."@en ;
	rdfs:range xsd:dateTime ;
	.

evidence:testimonyDate
	a owl:DatatypeProperty ;
	rdfs:label "testimonyDate"@en ;
	rdfs:comment "The date when the testimony was given."@en ;
	rdfs:range xsd:dateTime ;
	.

evidence:testimonyOrigin
	a owl:DatatypeProperty ;
	rdfs:label "testimonyOrigin"@en ;
	rdfs:comment "The individual that provided the testimony."@en ;
	rdfs:range xsd:string ;
	.

evidence:unixProcessName
	a owl:DatatypeProperty ;
	rdfs:label "unixProcessName"@en ;
	rdfs:comment "Name of the Unix process that is running in the list of processes. This could be placed inside uco-observable in future."@en ;
	rdfs:range xsd:string ;
	.

