# imports: https://ontology.unifiedcyberontology.org/uco/observable/1.1.0

@prefix indicators: <https://ontology.scopeontology.org/scope/indicators/> .
@prefix observable: <https://ontology.unifiedcyberontology.org/uco/observable/> .
@prefix owl: <http://www.w3.org/2002/07/owl#> .
@prefix rdf: <http://www.w3.org/1999/02/22-rdf-syntax-ns#> .
@prefix rdfs: <http://www.w3.org/2000/01/rdf-schema#> .
@prefix sh: <http://www.w3.org/ns/shacl#> .
@prefix xsd: <http://www.w3.org/2001/XMLSchema#> .

<https://ontology.scopeontology.org/scope/indicators>
	a owl:Ontology ;
	rdfs:label "scope-indicators"@en ;
	rdfs:comment "This ontology defines the indicators used in Smart City Infrastructure (SCI). For a more detailed explanation on how the indicators are grouped, please refer to the paper (https://doi.org/10.48550/arxiv.2210.14692). For ease of reference, the indicators are specified by their respective ISO clause number and comments specifying the details of the indicator."@en ;
	owl:imports observable:1.1.0 ;
	owl:versionIRI indicators:0.1.0 ;
	.

	
indicators:CitizenServiceSystemIndicator
	a
		owl:Class ,
		sh:NodeShape
		;
	rdfs:subClassOf indicators:Indicator ;
	rdfs:label "CitizenServiceSystemIndicator"@en ;
	rdfs:comment "A set of indicators that is classified under Citizen Service System, and contains various indicators from ISO 37120:2018, ISO 37122:2019 and ISO 37123:2019. For indicators stated in ISO 37120:2018, there are 3 further types of indicators - core, supporting and profile. Further details of these types of indicators are located at clause 3.4 of ISO 37120:2018."@en ;
	sh:targetClass indicators:CitizenServiceSystemIndicator ;
	.

indicators:Indicator
	a
		owl:Class ,
		sh:NodeShape
		;
	rdfs:subClassOf observable:ObservableObject ;
	rdfs:label "Indicator"@en ;
	rdfs:comment "An indicator is a quantitative, qualitative or descriptive measure (ISO 15392:2008)."@en ;
	sh:targetClass indicators:Indicator ;
	.


indicators:EconomyIndicator
	a
		owl:Class ,
		sh:NodeShape
		;
	rdfs:subClassOf indicators:CitizenServiceSystemIndicator ;
	rdfs:label "EconomyIndicator"@en ;
	rdfs:comment "A set of indicators that is classified under Citizen Service System, and contains various indicators under clause 5 from ISO 37120:2018, ISO 37122:2019 and ISO 37123:2019. For indicators stated in ISO 37120:2018, there are 3 further types of indicators - core, supporting and profile. Further details of these types of indicators are located at clause 3.4 of ISO 37120:2018."@en ;
	sh:targetClass indicators:EconomyIndicator ;
	.

indicators:EducationIndicator
	a
		owl:Class ,
		sh:NodeShape
		;
	rdfs:subClassOf indicators:CitizenServiceSystemIndicator ;
	rdfs:label "EducationIndicator"@en ;
	rdfs:comment "A set of indicators that is classified under Citizen Service System, and contains various indicators under clause 6 from ISO 37120:2018, ISO 37122:2019 and ISO 37123:2019. For indicators stated in ISO 37120:2018, there are 3 further types of indicators - core, supporting and profile. Further details of these types of indicators are located at clause 3.4 of ISO 37120:2018."@en ;
	sh:targetClass indicators:EducationIndicator ;
	.

indicators:EnergyIndicator
	a
		owl:Class ,
		sh:NodeShape
		;
	rdfs:subClassOf indicators:ResourceSystemIndicator ;
	rdfs:label "EnergyIndicator"@en ;
	rdfs:comment "A set of indicators that is classified under Resource System, and contains various indicators under clause 7 from ISO 37120:2018, ISO 37122:2019 and ISO 37123:2019. For indicators stated in ISO 37120:2018, there are 3 further types of indicators - core, supporting and profile. Further details of these types of indicators are located at clause 3.4 of ISO 37120:2018."@en ;
	sh:targetClass indicators:EnergyIndicator ;
	.

indicators:EnvironmentAndClimateChangeIndicator
	a
		owl:Class ,
		sh:NodeShape
		;
	rdfs:subClassOf indicators:LivelihoodSupportSystemIndicator ;
	rdfs:label "EnvironmentAndClimateChangeIndicator"@en ;
	rdfs:comment "A set of indicators that is classified under Livelihood Support System, and contains various indicators under clause 8 from ISO 37120:2018, ISO 37122:2019 and ISO 37123:2019. For indicators stated in ISO 37120:2018, there are 3 further types of indicators - core, supporting and profile. Further details of these types of indicators are located at clause 3.4 of ISO 37120:2018."@en ;
	sh:targetClass indicators:EnvironmentAndClimateChangeIndicator ;
	.

indicators:EssentialServiceSystemIndicator
	a
		owl:Class ,
		sh:NodeShape
		;
	rdfs:subClassOf indicators:Indicator ;
	rdfs:label "EssentialServiceSystemIndicator"@en ;
	rdfs:comment "A set of indicators that is classified under Essential Service System, and contains various indicators from ISO 37120:2018, ISO 37122:2019 and ISO 37123:2019. For indicators stated in ISO 37120:2018, there are 3 further types of indicators - core, supporting and profile. Further details of these types of indicators are located at clause 3.4 of ISO 37120:2018."@en ;
	sh:targetClass indicators:EssentialServiceSystemIndicator ;
	.

indicators:FinanceIndicator
	a
		owl:Class ,
		sh:NodeShape
		;
	rdfs:subClassOf indicators:CitizenServiceSystemIndicator ;
	rdfs:label "FinanceIndicator"@en ;
	rdfs:comment "A set of indicators that is classified under Citizen Service System, and contains various indicators under clause 9 from ISO 37120:2018, ISO 37122:2019 and ISO 37123:2019. For indicators stated in ISO 37120:2018, there are 3 further types of indicators - core, supporting and profile. Further details of these types of indicators are located at clause 3.4 of ISO 37120:2018."@en ;
	sh:targetClass indicators:FinanceIndicator ;
	.

indicators:GovernanceIndicator
	a
		owl:Class ,
		sh:NodeShape
		;
	rdfs:subClassOf indicators:CitizenServiceSystemIndicator ;
	rdfs:label "GovernanceIndicator"@en ;
	rdfs:comment "A set of indicators that is classified under Citizen Service System, and contains various indicators under clause 10 from ISO 37120:2018, ISO 37122:2019 and ISO 37123:2019. For indicators stated in ISO 37120:2018, there are 3 further types of indicators - core, supporting and profile. Further details of these types of indicators are located at clause 3.4 of ISO 37120:2018."@en ;
	sh:targetClass indicators:GovernanceIndicator ;
	.

indicators:HealthIndicator
	a
		owl:Class ,
		sh:NodeShape
		;
	rdfs:subClassOf indicators:EssentialServiceSystemIndicator ;
	rdfs:label "HealthIndicator"@en ;
	rdfs:comment "A set of indicators that is classified under Essential Service System, and contains various indicators under clause 11 from ISO 37120:2018, ISO 37122:2019 and ISO 37123:2019. For indicators stated in ISO 37120:2018, there are 3 further types of indicators - core, supporting and profile. Further details of these types of indicators are located at clause 3.4 of ISO 37120:2018."@en ;
	sh:targetClass indicators:HealthIndicator ;
	.

indicators:HousingIndicator
	a
		owl:Class ,
		sh:NodeShape
		;
	rdfs:subClassOf indicators:CitizenServiceSystemIndicator ;
	rdfs:label "HousingIndicator"@en ;
	rdfs:comment "A set of indicators that is classified under Citizen Service System, and contains various indicators under clause 12 from ISO 37120:2018, ISO 37122:2019 and ISO 37123:2019. For indicators stated in ISO 37120:2018, there are 3 further types of indicators - core, supporting and profile. Further details of these types of indicators are located at clause 3.4 of ISO 37120:2018."@en ;
	sh:targetClass indicators:HousingIndicator ;
	.

indicators:ISO37120ClauseEightPointEight
	a
		owl:Class ,
		sh:NodeShape
		;
	rdfs:subClassOf indicators:EnvironmentAndClimateChangeIndicator ;
	rdfs:label "ISO37120ClauseEightPointEight"@en ;
	rdfs:comment "ISO 37120:2018 Clause 8.8 - Noise pollution (supporting indicator)."@en ;
	sh:targetClass indicators:ISO37120ClauseEightPointEight ;
	.

indicators:ISO37120ClauseEightPointFive
	a
		owl:Class ,
		sh:NodeShape
		;
	rdfs:subClassOf indicators:EnvironmentAndClimateChangeIndicator ;
	rdfs:label "ISO37120ClauseEightPointFive"@en ;
	rdfs:comment "ISO 37120:2018 Clause 8.5 - NO2 (nitrogen dioxide) concentration (supporting indicator)."@en ;
	sh:targetClass indicators:ISO37120ClauseEightPointFive ;
	.

indicators:ISO37120ClauseEightPointFour
	a
		owl:Class ,
		sh:NodeShape
		;
	rdfs:subClassOf indicators:EnvironmentAndClimateChangeIndicator ;
	rdfs:label "ISO37120ClauseEightPointFour"@en ;
	rdfs:comment "ISO 37120:2018 Clause 8.4 - Percentage of areas designated for natural protection (supporting indicator)."@en ;
	sh:targetClass indicators:ISO37120ClauseEightPointFour ;
	.

indicators:ISO37120ClauseEightPointNine
	a
		owl:Class ,
		sh:NodeShape
		;
	rdfs:subClassOf indicators:EnvironmentAndClimateChangeIndicator ;
	rdfs:label "ISO37120ClauseEightPointNine"@en ;
	rdfs:comment "ISO 37120:2018 Clause 8.9 - Percentage change in number of native species (supporting indicator)."@en ;
	sh:targetClass indicators:ISO37120ClauseEightPointNine ;
	.

indicators:ISO37120ClauseEightPointOne
	a
		owl:Class ,
		sh:NodeShape
		;
	rdfs:subClassOf indicators:EnvironmentAndClimateChangeIndicator ;
	rdfs:label "ISO37120ClauseEightPointOne"@en ;
	rdfs:comment "ISO 37120:2018 Clause 8.1 - Fine particulate matter (PM2.5) concentration (core indicator)."@en ;
	sh:targetClass indicators:ISO37120ClauseEightPointOne ;
	.

indicators:ISO37120ClauseEightPointSeven
	a
		owl:Class ,
		sh:NodeShape
		;
	rdfs:subClassOf indicators:EnvironmentAndClimateChangeIndicator ;
	rdfs:label "ISO37120ClauseEightPointSeven"@en ;
	rdfs:comment "ISO 37120:2018 Clause 8.7 - O3 (ozone) concentration (supporting indicator)."@en ;
	sh:targetClass indicators:ISO37120ClauseEightPointSeven ;
	.

indicators:ISO37120ClauseEightPointSix
	a
		owl:Class ,
		sh:NodeShape
		;
	rdfs:subClassOf indicators:EnvironmentAndClimateChangeIndicator ;
	rdfs:label "ISO37120ClauseEightPointSix"@en ;
	rdfs:comment "ISO 37120:2018 Clause 8.6 - SO2 (sulfur dioxide) concentration (supporting indicator)."@en ;
	sh:targetClass indicators:ISO37120ClauseEightPointSix ;
	.

indicators:ISO37120ClauseEightPointThree
	a
		owl:Class ,
		sh:NodeShape
		;
	rdfs:subClassOf indicators:EnvironmentAndClimateChangeIndicator ;
	rdfs:label "ISO37120ClauseEightPointThree"@en ;
	rdfs:comment "ISO 37120:2018 Clause 8.3 - Greenhouse gas emissions measured in tonnes per capita (core indicator)."@en ;
	sh:targetClass indicators:ISO37120ClauseEightPointThree ;
	.

indicators:ISO37120ClauseEightPointTwo
	a
		owl:Class ,
		sh:NodeShape
		;
	rdfs:subClassOf indicators:EnvironmentAndClimateChangeIndicator ;
	rdfs:label "ISO37120ClauseEightPointTwo"@en ;
	rdfs:comment "ISO 37120:2018 Clause 8.2 - Particulate matter (PM10) concentration (core indicator)."@en ;
	sh:targetClass indicators:ISO37120ClauseEightPointTwo ;
	.

indicators:ISO37120ClauseEighteenPointOne
	a
		owl:Class ,
		sh:NodeShape
		;
	rdfs:subClassOf indicators:TelecommunicationIndicator ;
	rdfs:label "ISO37120ClauseEighteenPointOne"@en ;
	rdfs:comment "ISO 37120:2018 Clause 18.1 - Number of internet connections per 100 000 population (supporting indicator)."@en ;
	sh:targetClass indicators:ISO37120ClauseEighteenPointOne ;
	.

indicators:ISO37120ClauseEighteenPointTwo
	a
		owl:Class ,
		sh:NodeShape
		;
	rdfs:subClassOf indicators:TelecommunicationIndicator ;
	rdfs:label "ISO37120ClauseEighteenPointTwo"@en ;
	rdfs:comment "ISO 37120:2018 Clause 18.2 - Number of mobile phone connections per 100 000 population (supporting indicator)."@en ;
	sh:targetClass indicators:ISO37120ClauseEighteenPointTwo ;
	.

indicators:ISO37120ClauseElevenPointFive
	a
		owl:Class ,
		sh:NodeShape
		;
	rdfs:subClassOf indicators:HealthIndicator ;
	rdfs:label "ISO37120ClauseElevenPointFive"@en ;
	rdfs:comment "ISO 37120:2018 Clause 11.5 - Number of nursing and midwifery personnel per 100 000 population (supporting indicator)."@en ;
	sh:targetClass indicators:ISO37120ClauseElevenPointFive ;
	.

indicators:ISO37120ClauseElevenPointFour
	a
		owl:Class ,
		sh:NodeShape
		;
	rdfs:subClassOf indicators:HealthIndicator ;
	rdfs:label "ISO37120ClauseElevenPointFour"@en ;
	rdfs:comment "ISO 37120:2018 Clause 11.4 - Under age five mortality per 1 000 live births (core indicator)."@en ;
	sh:targetClass indicators:ISO37120ClauseElevenPointFour ;
	.

indicators:ISO37120ClauseElevenPointOne
	a
		owl:Class ,
		sh:NodeShape
		;
	rdfs:subClassOf indicators:HealthIndicator ;
	rdfs:label "ISO37120ClauseElevenPointOne"@en ;
	rdfs:comment "ISO 37120:2018 Clause 11.1 - Average life expectancy (core indicator)."@en ;
	sh:targetClass indicators:ISO37120ClauseElevenPointOne ;
	.

indicators:ISO37120ClauseElevenPointSix
	a
		owl:Class ,
		sh:NodeShape
		;
	rdfs:subClassOf indicators:HealthIndicator ;
	rdfs:label "ISO37120ClauseElevenPointSix"@en ;
	rdfs:comment "ISO 37120:2018 Clause 11.6 - Suicide rate per 100 000 population (supporting indicator)."@en ;
	sh:targetClass indicators:ISO37120ClauseElevenPointSix ;
	.

indicators:ISO37120ClauseElevenPointThree
	a
		owl:Class ,
		sh:NodeShape
		;
	rdfs:subClassOf indicators:HealthIndicator ;
	rdfs:label "ISO37120ClauseElevenPointThree"@en ;
	rdfs:comment "ISO 37120:2018 Clause 11.3 - Number of physicians per 100 000 population (core indicator)."@en ;
	sh:targetClass indicators:ISO37120ClauseElevenPointThree ;
	.

indicators:ISO37120ClauseElevenPointTwo
	a
		owl:Class ,
		sh:NodeShape
		;
	rdfs:subClassOf indicators:HealthIndicator ;
	rdfs:label "ISO37120ClauseElevenPointTwo"@en ;
	rdfs:comment "ISO 37120:2018 Clause 11.2 - Number of in-patient hospital beds per 100 000 population (core indicator)."@en ;
	sh:targetClass indicators:ISO37120ClauseElevenPointTwo ;
	.

indicators:ISO37120ClauseFifteenPointEight
	a
		owl:Class ,
		sh:NodeShape
		;
	rdfs:subClassOf indicators:SafetyIndicator ;
	rdfs:label "ISO37120ClauseFifteenPointEight"@en ;
	rdfs:comment "ISO 37120:2018 Clause 15.8 - Crimes against property per 100 000 population (supporting indicator)."@en ;
	sh:targetClass indicators:ISO37120ClauseFifteenPointEight ;
	.

indicators:ISO37120ClauseFifteenPointFive
	a
		owl:Class ,
		sh:NodeShape
		;
	rdfs:subClassOf indicators:SafetyIndicator ;
	rdfs:label "ISO37120ClauseFifteenPointFive"@en ;
	rdfs:comment "ISO 37120:2018 Clause 15.5 - Number of homicides per 100 000 population (core indicator)."@en ;
	sh:targetClass indicators:ISO37120ClauseFifteenPointFive ;
	.

indicators:ISO37120ClauseFifteenPointFour
	a
		owl:Class ,
		sh:NodeShape
		;
	rdfs:subClassOf indicators:SafetyIndicator ;
	rdfs:label "ISO37120ClauseFifteenPointFour"@en ;
	rdfs:comment "ISO 37120:2018 Clause 15.4 - Number of police officers per 100 000 population (core indicator)."@en ;
	sh:targetClass indicators:ISO37120ClauseFifteenPointFour ;
	.

indicators:ISO37120ClauseFifteenPointNine
	a
		owl:Class ,
		sh:NodeShape
		;
	rdfs:subClassOf indicators:SafetyIndicator ;
	rdfs:label "ISO37120ClauseFifteenPointNine"@en ;
	rdfs:comment "ISO 37120:2018 Clause 15.9 - Number of deaths caused by industrial accidents per 100 000 population (supporting indicator)."@en ;
	sh:targetClass indicators:ISO37120ClauseFifteenPointNine ;
	.

indicators:ISO37120ClauseFifteenPointOne
	a
		owl:Class ,
		sh:NodeShape
		;
	rdfs:subClassOf indicators:SafetyIndicator ;
	rdfs:label "ISO37120ClauseFifteenPointOne"@en ;
	rdfs:comment "ISO 37120:2018 Clause 15.1 - Number of firefighters per 100 000 population (core indicator)."@en ;
	sh:targetClass indicators:ISO37120ClauseFifteenPointOne ;
	.

indicators:ISO37120ClauseFifteenPointSeven
	a
		owl:Class ,
		sh:NodeShape
		;
	rdfs:subClassOf indicators:SafetyIndicator ;
	rdfs:label "ISO37120ClauseFifteenPointSeven"@en ;
	rdfs:comment "ISO 37120:2018 Clause 15.7 - Response time for emergency response services from initial call (supporting indicator)."@en ;
	sh:targetClass indicators:ISO37120ClauseFifteenPointSeven ;
	.

indicators:ISO37120ClauseFifteenPointSix
	a
		owl:Class ,
		sh:NodeShape
		;
	rdfs:subClassOf indicators:SafetyIndicator ;
	rdfs:label "ISO37120ClauseFifteenPointSix"@en ;
	rdfs:comment "ISO 37120:2018 Clause 15.6 -	Number of volunteer and part-time firefighters per 100 000 population (supporting indicator)."@en ;
	sh:targetClass indicators:ISO37120ClauseFifteenPointSix ;
	.

indicators:ISO37120ClauseFifteenPointTen
	a
		owl:Class ,
		sh:NodeShape
		;
	rdfs:subClassOf indicators:SafetyIndicator ;
	rdfs:label "ISO37120ClauseFifteenPointTen"@en ;
	rdfs:comment "ISO 37120:2018 Clause 15.10 - Number of violent crimes against women per 100 000 population (supporting indicator)."@en ;
	sh:targetClass indicators:ISO37120ClauseFifteenPointTen ;
	.

indicators:ISO37120ClauseFifteenPointThree
	a
		owl:Class ,
		sh:NodeShape
		;
	rdfs:subClassOf indicators:SafetyIndicator ;
	rdfs:label "ISO37120ClauseFifteenPointThree"@en ;
	rdfs:comment "ISO 37120:2018 Clause 15.3 - Number of natural-hazard-related deaths per 100 000 population (core indicator)."@en ;
	sh:targetClass indicators:ISO37120ClauseFifteenPointThree ;
	.

indicators:ISO37120ClauseFifteenPointTwo
	a
		owl:Class ,
		sh:NodeShape
		;
	rdfs:subClassOf indicators:SafetyIndicator ;
	rdfs:label "ISO37120ClauseFifteenPointTwo"@en ;
	rdfs:comment "ISO 37120:2018 Clause 15.2 - Number of fire-related deaths per 100 000 population (core indicator)."@en ;
	sh:targetClass indicators:ISO37120ClauseFifteenPointTwo ;
	.

indicators:ISO37120ClauseFivePointEight
	a
		owl:Class ,
		sh:NodeShape
		;
	rdfs:subClassOf indicators:EconomyIndicator ;
	rdfs:label "ISO37120ClauseFivePointEight"@en ;
	rdfs:comment "ISO 37120:2018 Clause 5.8 - Commercial air connectivity (number of non-stop commercial air destinations) (supporting indicator)."@en ;
	sh:targetClass indicators:ISO37120ClauseFivePointEight ;
	.

indicators:ISO37120ClauseFivePointFive
	a
		owl:Class ,
		sh:NodeShape
		;
	rdfs:subClassOf indicators:EconomyIndicator ;
	rdfs:label "ISO37120ClauseFivePointFive"@en ;
	rdfs:comment "ISO 37120:2018 Clause 5.5 - Number of businesses per 100 000 population (supporting indicator)."@en ;
	sh:targetClass indicators:ISO37120ClauseFivePointFive ;
	.

indicators:ISO37120ClauseFivePointFour
	a
		owl:Class ,
		sh:NodeShape
		;
	rdfs:subClassOf indicators:EconomyIndicator ;
	rdfs:label "ISO37120ClauseFivePointFour"@en ;
	rdfs:comment "ISO 37120:2018 Clause 5.4 - Youth unemployment rate (supporting indicator)."@en ;
	sh:targetClass indicators:ISO37120ClauseFivePointFour ;
	.

indicators:ISO37120ClauseFivePointNinePointOne
	a
		owl:Class ,
		sh:NodeShape
		;
	rdfs:subClassOf indicators:EconomyIndicator ;
	rdfs:label "ISO37120ClauseFivePointNinePointOne"@en ;
	rdfs:comment "ISO 37120:2018 Clause 5.9.1 - Average household income (USD) (profile indicator)."@en ;
	sh:targetClass indicators:ISO37120ClauseFivePointNinePointOne ;
	.

indicators:ISO37120ClauseFivePointNinePointThree
	a
		owl:Class ,
		sh:NodeShape
		;
	rdfs:subClassOf indicators:EconomyIndicator ;
	rdfs:label "ISO37120ClauseFivePointNinePointThree"@en ;
	rdfs:comment "ISO 37120:2018 Clause 5.9.3 - City product per capita (USD) (profile indicator)."@en ;
	sh:targetClass indicators:ISO37120ClauseFivePointNinePointThree ;
	.

indicators:ISO37120ClauseFivePointNinePointTwo
	a
		owl:Class ,
		sh:NodeShape
		;
	rdfs:subClassOf indicators:EconomyIndicator ;
	rdfs:label "ISO37120ClauseFivePointNinePointTwo"@en ;
	rdfs:comment "ISO 37120:2018 Clause 5.9.2 - Annual inflation rate based on the average of the past five years (profile indicator)."@en ;
	sh:targetClass indicators:ISO37120ClauseFivePointNinePointTwo ;
	.

indicators:ISO37120ClauseFivePointOne
	a
		owl:Class ,
		sh:NodeShape
		;
	rdfs:subClassOf indicators:EconomyIndicator ;
	rdfs:label "ISO37120ClauseFivePointOne"@en ;
	rdfs:comment "ISO 37120:2018 Clause 5.1 - City’s unemployment rate (core indicator)."@en ;
	sh:targetClass indicators:ISO37120ClauseFivePointOne ;
	.

indicators:ISO37120ClauseFivePointSeven
	a
		owl:Class ,
		sh:NodeShape
		;
	rdfs:subClassOf indicators:EconomyIndicator ;
	rdfs:label "ISO37120ClauseFivePointSeven"@en ;
	rdfs:comment "ISO 37120:2018 Clause 5.7 - Annual number of visitor stays (overnight) per 100 000 population (supporting indicator)."@en ;
	sh:targetClass indicators:ISO37120ClauseFivePointSeven ;
	.

indicators:ISO37120ClauseFivePointSix
	a
		owl:Class ,
		sh:NodeShape
		;
	rdfs:subClassOf indicators:EconomyIndicator ;
	rdfs:label "ISO37120ClauseFivePointSix"@en ;
	rdfs:comment "ISO 37120:2018 Clause 5.6 - Number of new patents per 100 000 population per year (supporting indicator)."@en ;
	sh:targetClass indicators:ISO37120ClauseFivePointSix ;
	.

indicators:ISO37120ClauseFivePointThree
	a
		owl:Class ,
		sh:NodeShape
		;
	rdfs:subClassOf indicators:EconomyIndicator ;
	rdfs:label "ISO37120ClauseFivePointThree"@en ;
	rdfs:comment "ISO 37120:2018 Clause 5.3 - Percentage of persons in full-time employment (supporting indicator)."@en ;
	sh:targetClass indicators:ISO37120ClauseFivePointThree ;
	.

indicators:ISO37120ClauseFivePointTwo
	a
		owl:Class ,
		sh:NodeShape
		;
	rdfs:subClassOf indicators:EconomyIndicator ;
	rdfs:label "ISO37120ClauseFivePointTwo"@en ;
	rdfs:comment "ISO 37120:2018 Clause 5.2 - Assessed value of commercial and industrial properties as a percentage of total assessed value of all properties (supporting indicator)."@en ;
	sh:targetClass indicators:ISO37120ClauseFivePointTwo ;
	.

indicators:ISO37120ClauseFourteenPointOne
	a
		owl:Class ,
		sh:NodeShape
		;
	rdfs:subClassOf indicators:RecreationIndicator ;
	rdfs:label "ISO37120ClauseFourteenPointOne"@en ;
	rdfs:comment "ISO 37120:2018 Clause 14.1 - Square metres of public indoor recreation space per capita (supporting indicator)."@en ;
	sh:targetClass indicators:ISO37120ClauseFourteenPointOne ;
	.

indicators:ISO37120ClauseFourteenPointTwo
	a
		owl:Class ,
		sh:NodeShape
		;
	rdfs:subClassOf indicators:RecreationIndicator ;
	rdfs:label "ISO37120ClauseFourteenPointTwo"@en ;
	rdfs:comment "ISO 37120:2018 Clause 14.2 - Square metres of public outdoor recreation space per capita (supporting indicator)."@en ;
	sh:targetClass indicators:ISO37120ClauseFourteenPointTwo ;
	.

indicators:ISO37120ClauseNinePointFivePointOne
	a
		owl:Class ,
		sh:NodeShape
		;
	rdfs:subClassOf indicators:FinanceIndicator ;
	rdfs:label "ISO37120ClauseNinePointFivePointOne"@en ;
	rdfs:comment "ISO 37120:2018 Clause 9.5.1 - Gross operating budget per capita (USD) (profile indicator)."@en ;
	sh:targetClass indicators:ISO37120ClauseNinePointFivePointOne ;
	.

indicators:ISO37120ClauseNinePointFivePointTwo
	a
		owl:Class ,
		sh:NodeShape
		;
	rdfs:subClassOf indicators:FinanceIndicator ;
	rdfs:label "ISO37120ClauseNinePointFivePointTwo"@en ;
	rdfs:comment "ISO 37120:2018 Clause 9.5.2 - Gross capital budget per capita (USD) (profile indicator)."@en ;
	sh:targetClass indicators:ISO37120ClauseNinePointFivePointTwo ;
	.

	indicators:ISO37120ClauseNinePointFour
	a
		owl:Class ,
		sh:NodeShape
		;
	rdfs:subClassOf indicators:FinanceIndicator ;
	rdfs:label "ISO37120ClauseNinePointFour"@en ;
	rdfs:comment "ISO 37120:2018 Clause 9.4 - Tax collected as a percentage of tax billed (supporting indicator)."@en ;
	sh:targetClass indicators:ISO37120ClauseNinePointFour ;
	.

indicators:ISO37120ClauseNinePointOne
	a
		owl:Class ,
		sh:NodeShape
		;
	rdfs:subClassOf indicators:FinanceIndicator ;
	rdfs:label "ISO37120ClauseNinePointOne"@en ;
	rdfs:comment "ISO 37120:2018 Clause 9.1 - Debt service ratio (debt service expenditure as a percentage of a city's own-source revenue) (core indicator)."@en ;
	sh:targetClass indicators:ISO37120ClauseNinePointOne ;
	.

indicators:ISO37120ClauseNinePointThree
	a
		owl:Class ,
		sh:NodeShape
		;
	rdfs:subClassOf indicators:FinanceIndicator ;
	rdfs:label "ISO37120ClauseNinePointThree"@en ;
	rdfs:comment "ISO 37120:2018 Clause 9.3 - Own-source revenue as a percentage of total revenues (supporting indicator)."@en ;
	sh:targetClass indicators:ISO37120ClauseNinePointThree ;
	.

indicators:ISO37120ClauseNinePointTwo
	a
		owl:Class ,
		sh:NodeShape
		;
	rdfs:subClassOf indicators:FinanceIndicator ;
	rdfs:label "ISO37120ClauseNinePointTwo"@en ;
	rdfs:comment "ISO 37120:2018 Clause 9.2 - Capital spending as a percentage of total expenditures (core indicator)."@en ;
	sh:targetClass indicators:ISO37120ClauseNinePointTwo ;
	.

indicators:ISO37120ClauseNineteenPointEightPointOne
	a
		owl:Class ,
		sh:NodeShape
		;
	rdfs:subClassOf indicators:TransportationIndicator ;
	rdfs:label "ISO37120ClauseEightPointEight"@en ;
	rdfs:comment "ISO 37120:2018 Clause 19.8.1 - Number of personal automobiles per capita (profile indicator)."@en ;
	sh:targetClass indicators:ISO37120ClauseEightPointEight ;
	.

indicators:ISO37120ClauseNineteenPointEightPointTwo
	a
		owl:Class ,
		sh:NodeShape
		;
	rdfs:subClassOf indicators:TransportationIndicator ;
	rdfs:label "ISO37120ClauseNineteenPointEightPointTwo"@en ;
	rdfs:comment "ISO 37120:2018 Clause 19.8.2 - Number of two-wheeled motorized vehicles per capita (profile indicator)."@en ;
	sh:targetClass indicators:ISO37120ClauseNineteenPointEightPointTwo ;
	.

indicators:ISO37120ClauseNineteenPointFive
	a
		owl:Class ,
		sh:NodeShape
		;
	rdfs:subClassOf indicators:TransportationIndicator ;
	rdfs:label "ISO37120ClauseNineteenPointFive"@en ;
	rdfs:comment "ISO 37120:2018 Clause 19.5 - Transportation deaths per 100 000 population (supporting indicator)."@en ;
	sh:targetClass indicators:ISO37120ClauseNineteenPointFive ;
	.

indicators:ISO37120ClauseNineteenPointFour
	a
		owl:Class ,
		sh:NodeShape
		;
	rdfs:subClassOf indicators:TransportationIndicator ;
	rdfs:label "ISO37120ClauseNineteenPointFour"@en ;
	rdfs:comment "ISO 37120:2018 Clause 19.4 - Kilometres of bicycle paths and lanes per 100 000 population (supporting indicator)."@en-gb ;
	sh:targetClass indicators:ISO37120ClauseNineteenPointFour ;
	.

indicators:ISO37120ClauseNineteenPointOne
	a
		owl:Class ,
		sh:NodeShape
		;
	rdfs:subClassOf indicators:TransportationIndicator ;
	rdfs:label "ISO37120ClauseNineteenPointOne"@en ;
	rdfs:comment "ISO 37120:2018 Clause 19.1 - Kilometres of public transport system per 100 000 population (core indicator)."@en-gb ;
	sh:targetClass indicators:ISO37120ClauseNineteenPointOne ;
	.

indicators:ISO37120ClauseNineteenPointSeven
	a
		owl:Class ,
		sh:NodeShape
		;
	rdfs:subClassOf indicators:TransportationIndicator ;
	rdfs:label "ISO37120ClauseNineteenPointSeven"@en ;
	rdfs:comment "ISO 37120:2018 Clause 19.7 - Noise pollution (supporting indicator)."@en ;
	sh:targetClass indicators:ISO37120ClauseNineteenPointSeven ;
	.

indicators:ISO37120ClauseNineteenPointSix
	a
		owl:Class ,
		sh:NodeShape
		;
	rdfs:subClassOf indicators:TransportationIndicator ;
	rdfs:label "ISO37120ClauseNineteenPointSix"@en ;
	rdfs:comment "ISO 37120:2018 Clause 19.6 - Percentage of population living within 0,5 km of public transit running at least every 20 min during peak periods (supporting indicator)."@en ;
	sh:targetClass indicators:ISO37120ClauseNineteenPointSix ;
	.

indicators:ISO37120ClauseNineteenPointThree
	a
		owl:Class ,
		sh:NodeShape
		;
	rdfs:subClassOf indicators:TransportationIndicator ;
	rdfs:label "ISO37120ClauseNineteenPointThree"@en ;
	rdfs:comment "ISO 37120:2018 Clause 19.3 - Percentage of commuters using a travel mode to work other than a personal vehicle (supporting indicator)."@en ;
	sh:targetClass indicators:ISO37120ClauseNineteenPointThree ;
	.

indicators:ISO37120ClauseNineteenPointTwo
	a
		owl:Class ,
		sh:NodeShape
		;
	rdfs:subClassOf indicators:TransportationIndicator ;
	rdfs:label "ISO37120ClauseNineteenPointTwo"@en ;
	rdfs:comment "ISO 37120:2018 Clause 19.2 - Annual number of public transport trips per capita (core indicator)."@en ;
	sh:targetClass indicators:ISO37120ClauseNineteenPointTwo ;
	.

indicators:ISO37120ClauseSevenPointEightPointOne
	a
		owl:Class ,
		sh:NodeShape
		;
	rdfs:subClassOf indicators:EnergyIndicator ;
	rdfs:label "ISO37120ClauseSevenPointEightPointOne"@en ;
	rdfs:comment "ISO 37120:2018 Clause 7.8.1 - Heating degree days (profile indicator)."@en ;
	sh:targetClass indicators:ISO37120ClauseSevenPointEightPointOne ;
	.

indicators:ISO37120ClauseSevenPointEightPointTwo
	a
		owl:Class ,
		sh:NodeShape
		;
	rdfs:subClassOf indicators:EnergyIndicator ;
	rdfs:label "ISO37120ClauseSevenPointEightPointTwo"@en ;
	rdfs:comment "ISO 37120:2018 Clause 7.8.2 - Cooling degree days (profile indicator)."@en ;
	sh:targetClass indicators:ISO37120ClauseSevenPointEightPointTwo ;
	.

indicators:ISO37120ClauseSevenPointFive
	a
		owl:Class ,
		sh:NodeShape
		;
	rdfs:subClassOf indicators:EnergyIndicator ;
	rdfs:label "ISO37120ClauseSevenPointFive"@en ;
	rdfs:comment "ISO 37120:2018 Clause 7.5 - Final energy consumption of public buildings per year (GJ/m2) (core indicator)."@en ;
	sh:targetClass indicators:ISO37120ClauseSevenPointFive ;
	.

indicators:ISO37120ClauseSevenPointFour
	a
		owl:Class ,
		sh:NodeShape
		;
	rdfs:subClassOf indicators:EnergyIndicator ;
	rdfs:label "ISO37120ClauseSevenPointFour"@en ;
	rdfs:comment "ISO 37120:2018 Clause 7.4 - Number of gas distribution service connections per 100 000 population (residential) (core indicator)."@en ;
	sh:targetClass indicators:ISO37120ClauseSevenPointFour ;
	.

indicators:ISO37120ClauseSevenPointOne
	a
		owl:Class ,
		sh:NodeShape
		;
	rdfs:subClassOf indicators:EnergyIndicator ;
	rdfs:label "ISO37120ClauseSevenPointOne"@en ;
	rdfs:comment "ISO 37120:2018 Clause 7.1 - Total end-use energy consumption per capita (GJ/year) (core indicator)."@en ;
	sh:targetClass indicators:ISO37120ClauseSevenPointOne ;
	.

indicators:ISO37120ClauseSevenPointSeven
	a
		owl:Class ,
		sh:NodeShape
		;
	rdfs:subClassOf indicators:EnergyIndicator ;
	rdfs:label "ISO37120ClauseSevenPointSeven"@en ;
	rdfs:comment "ISO 37120:2018 Clause 7.7 - Average annual hours of electrical service interruptions per household (supporting indicator)."@en ;
	sh:targetClass indicators:ISO37120ClauseSevenPointSeven ;
	.

indicators:ISO37120ClauseSevenPointSix
	a
		owl:Class ,
		sh:NodeShape
		;
	rdfs:subClassOf indicators:EnergyIndicator ;
	rdfs:label "ISO37120ClauseSevenPointSix"@en ;
	rdfs:comment "ISO 37120:2018 Clause 7.6 - Electricity consumption of public street lighting per kilometre of lighted street (kWh/year) (supporting indicator)."@en-gb ;
	sh:targetClass indicators:ISO37120ClauseSevenPointSix ;
	.

indicators:ISO37120ClauseSevenPointThree
	a
		owl:Class ,
		sh:NodeShape
		;
	rdfs:subClassOf indicators:EnergyIndicator ;
	rdfs:label "ISO37120ClauseSevenPointThree"@en ;
	rdfs:comment "ISO 37120:2018 Clause 7.3 - Percentage of city population with authorized electrical service (residential) (core indicator)."@en-us ;
	sh:targetClass indicators:ISO37120ClauseSevenPointThree ;
	.

indicators:ISO37120ClauseSevenPointTwo
	a
		owl:Class ,
		sh:NodeShape
		;
	rdfs:subClassOf indicators:EnergyIndicator ;
	rdfs:label "ISO37120ClauseSevenPointTwo"@en ;
	rdfs:comment "ISO 37120:2018 Clause 7.2 - Percentage of total end-use energy derived from renewable sources (core indicator)."@en ;
	sh:targetClass indicators:ISO37120ClauseSevenPointTwo ;
	.

indicators:ISO37120ClauseSeventeenPointOne
	a
		owl:Class ,
		sh:NodeShape
		;
	rdfs:subClassOf indicators:SportAndCultureIndicator ;
	rdfs:label "ISO37120ClauseSeventeenPointOne"@en ;
	rdfs:comment "ISO 37120:2018 Clause 17.1 - Number of cultural institutions and sporting facilities per 100 000 population (core indicator)."@en ;
	sh:targetClass indicators:ISO37120ClauseSeventeenPointOne ;
	.

indicators:ISO37120ClauseSeventeenPointThree
	a
		owl:Class ,
		sh:NodeShape
		;
	rdfs:subClassOf indicators:SportAndCultureIndicator ;
	rdfs:label "ISO37120ClauseSeventeenPointThree"@en ;
	rdfs:comment "ISO 37120:2018 Clause 17.3 - Annual number of cultural events per 100 000 population (e.g. exhibitions, festivals, concerts) (supporting indicator)."@en ;
	sh:targetClass indicators:ISO37120ClauseSeventeenPointThree ;
	.

indicators:ISO37120ClauseSeventeenPointTwo
	a
		owl:Class ,
		sh:NodeShape
		;
	rdfs:subClassOf indicators:SportAndCultureIndicator ;
	rdfs:label "ISO37120ClauseSeventeenPointTwo"@en ;
	rdfs:comment "ISO 37120:2018 Clause 17.2 - Percentage of municipal budget allocated to cultural and sporting facilities (supporting indicator)."@en ;
	sh:targetClass indicators:ISO37120ClauseSeventeenPointTwo ;
	.

indicators:ISO37120ClauseSixPointFive
	a
		owl:Class ,
		sh:NodeShape
		;
	rdfs:subClassOf indicators:EducationIndicator ;
	rdfs:label "ISO37120ClauseSixPointFive"@en ;
	rdfs:comment "ISO 37120:2018 Clause 6.5 - Percentage of school-aged population enrolled in schools (supporting indicator)."@en ;
	sh:targetClass indicators:ISO37120ClauseSixPointFive ;
	.

indicators:ISO37120ClauseSixPointFour
	a
		owl:Class ,
		sh:NodeShape
		;
	rdfs:subClassOf indicators:EducationIndicator ;
	rdfs:label "ISO37120ClauseSixPointFour"@en ;
	rdfs:comment "ISO 37120:2018 Clause 6.4 - Primary education student–teacher ratio (core indicator)."@en ;
	sh:targetClass indicators:ISO37120ClauseSixPointFour ;
	.

indicators:ISO37120ClauseSixPointOne
	a
		owl:Class ,
		sh:NodeShape
		;
	rdfs:subClassOf indicators:EducationIndicator ;
	rdfs:label "ISO37120ClauseSixPointOne"@en ;
	rdfs:comment "ISO 37120:2018 Clause 6.1 - Percentage of female school-aged population enrolled in schools (core indicator)."@en ;
	sh:targetClass indicators:ISO37120ClauseSixPointOne ;
	.

indicators:ISO37120ClauseSixPointSix
	a
		owl:Class ,
		sh:NodeShape
		;
	rdfs:subClassOf indicators:EducationIndicator ;
	rdfs:label "ISO37120ClauseSixPointSix"@en ;
	rdfs:comment "ISO 37120:2018 Clause 6.6 - Number of higher education degrees per 100 000 population (supporting indicator)."@en ;
	sh:targetClass indicators:ISO37120ClauseSixPointSix ;
	.

indicators:ISO37120ClauseSixPointThree
	a
		owl:Class ,
		sh:NodeShape
		;
	rdfs:subClassOf indicators:EducationIndicator ;
	rdfs:label "ISO37120ClauseSixPointThree"@en ;
	rdfs:comment "ISO 37120:2018 Clause 6.3 - Percentage of students completing secondary education: survival rate (core indicator)."@en ;
	sh:targetClass indicators:ISO37120ClauseSixPointThree ;
	.

indicators:ISO37120ClauseSixPointTwo
	a
		owl:Class ,
		sh:NodeShape
		;
	rdfs:subClassOf indicators:EducationIndicator ;
	rdfs:label "ISO37120ClauseSixPointTwo"@en ;
	rdfs:comment "ISO 37120:2018 Clause 6.2 - Percentage of students completing primary education: survival rate (core indicator)."@en ;
	sh:targetClass indicators:ISO37120ClauseSixPointTwo ;
	.

indicators:ISO37120ClauseSixteenPointEight
	a
		owl:Class ,
		sh:NodeShape
		;
	rdfs:subClassOf indicators:SolidWasteIndicator ;
	rdfs:label "ISO37120ClauseSixteenPointEight"@en ;
	rdfs:comment "ISO 37120:2018 Clause 16.8 - Percentage of the city's solid waste that is disposed of by other means (supporting indicator)."@en ;
	sh:targetClass indicators:ISO37120ClauseSixteenPointEight ;
	.

indicators:ISO37120ClauseSixteenPointFive
	a
		owl:Class ,
		sh:NodeShape
		;
	rdfs:subClassOf indicators:SolidWasteIndicator ;
	rdfs:label "ISO37120ClauseSixteenPointFive"@en ;
	rdfs:comment "ISO 37120:2018 Clause 16.5 - Percentage of the city's solid waste that is treated in energy-from-waste plants (core indicator)."@en ;
	sh:targetClass indicators:ISO37120ClauseSixteenPointFive ;
	.

indicators:ISO37120ClauseSixteenPointFour
	a
		owl:Class ,
		sh:NodeShape
		;
	rdfs:subClassOf indicators:SolidWasteIndicator ;
	rdfs:label "ISO37120ClauseSixteenPointFour"@en ;
	rdfs:comment "ISO 37120:2018 Clause 16.4 - Percentage of the city's solid waste that is disposed of in a sanitary landfill (core indicator)."@en ;
	sh:targetClass indicators:ISO37120ClauseSixteenPointFour ;
	.

indicators:ISO37120ClauseSixteenPointNine
	a
		owl:Class ,
		sh:NodeShape
		;
	rdfs:subClassOf indicators:SolidWasteIndicator ;
	rdfs:label "ISO37120ClauseSixteenPointNine"@en ;
	rdfs:comment "ISO 37120:2018 Clause 16.9 - Hazardous waste generation per capita (tonnes) (supporting indicator)."@en-gb ;
	sh:targetClass indicators:ISO37120ClauseSixteenPointNine ;
	.

indicators:ISO37120ClauseSixteenPointOne
	a
		owl:Class ,
		sh:NodeShape
		;
	rdfs:subClassOf indicators:SolidWasteIndicator ;
	rdfs:label "ISO37120ClauseSixteenPointOne"@en ;
	rdfs:comment "ISO 37120:2018 Clause 16.1 - Percentage of city population with regular solid waste collection (residential) (core indicator)."@en ;
	sh:targetClass indicators:ISO37120ClauseSixteenPointOne ;
	.

indicators:ISO37120ClauseSixteenPointSeven
	a
		owl:Class ,
		sh:NodeShape
		;
	rdfs:subClassOf indicators:SolidWasteIndicator ;
	rdfs:label "ISO37120ClauseSixteenPointSeven"@en ;
	rdfs:comment "ISO 37120:2018 Clause 16.7 - Percentage of the city's solid waste that is disposed of in an open dump (supporting indicator)."@en ;
	sh:targetClass indicators:ISO37120ClauseSixteenPointSeven ;
	.

indicators:ISO37120ClauseSixteenPointSix
	a
		owl:Class ,
		sh:NodeShape
		;
	rdfs:subClassOf indicators:SolidWasteIndicator ;
	rdfs:label "ISO37120ClauseSixteenPointSix"@en ;
	rdfs:comment "ISO 37120:2018 Clause 16.6 - Percentage of the city's solid waste that is biologically treated and used as compost or biogas (supporting indicator)."@en ;
	sh:targetClass indicators:ISO37120ClauseSixteenPointSix ;
	.

indicators:ISO37120ClauseSixteenPointTen
	a
		owl:Class ,
		sh:NodeShape
		;
	rdfs:subClassOf indicators:SolidWasteIndicator ;
	rdfs:label "ISO37120ClauseSixteenPointTen"@en ;
	rdfs:comment "ISO 37120:2018 Clause 16.10 - Percentage of the city’s hazardous waste that is recycled (supporting indicator)."@en ;
	sh:targetClass indicators:ISO37120ClauseSixteenPointTen ;
	.

indicators:ISO37120ClauseSixteenPointThree
	a
		owl:Class ,
		sh:NodeShape
		;
	rdfs:subClassOf indicators:SolidWasteIndicator ;
	rdfs:label "ISO37120ClauseSixteenPointThree"@en ;
	rdfs:comment "ISO 37120:2018 Clause 16.3 - Percentage of the city's solid waste that is recycled (core indicator)."@en ;
	sh:targetClass indicators:ISO37120ClauseSixteenPointThree ;
	.

indicators:ISO37120ClauseSixteenPointTwo
	a
		owl:Class ,
		sh:NodeShape
		;
	rdfs:subClassOf indicators:SolidWasteIndicator ;
	rdfs:label "ISO37120ClauseSixteenPointTwo"@en ;
	rdfs:comment "ISO 37120:2018 Clause 16.2 - Total collected municipal solid waste per capita (core indicator)."@en ;
	sh:targetClass indicators:ISO37120ClauseSixteenPointTwo ;
	.

indicators:ISO37120ClauseTenPointFour
	a
		owl:Class ,
		sh:NodeShape
		;
	rdfs:subClassOf indicators:GovernanceIndicator ;
	rdfs:label "ISO37120ClauseTenPointFour"@en ;
	rdfs:comment "ISO 37120:2018 Clause 10.4 - Voter participation in last municipal election (as a percentage of registered voters) (supporting indicator)."@en ;
	sh:targetClass indicators:ISO37120ClauseTenPointFour ;
	.

indicators:ISO37120ClauseTenPointOne
	a
		owl:Class ,
		sh:NodeShape
		;
	rdfs:subClassOf indicators:GovernanceIndicator ;
	rdfs:label "ISO37120ClauseTenPointOne"@en ;
	rdfs:comment "ISO 37120:2018 Clause 10.1 - Women as a percentage of total elected to city-level office (core indicator)."@en ;
	sh:targetClass indicators:ISO37120ClauseTenPointOne ;
	.

indicators:ISO37120ClauseTenPointThree
	a
		owl:Class ,
		sh:NodeShape
		;
	rdfs:subClassOf indicators:GovernanceIndicator ;
	rdfs:label "ISO37120ClauseTenPointThree"@en ;
	rdfs:comment "ISO 37120:2018 Clause 10.3 - Number of registered voters as a percentage of the voting age population (supporting indicator)."@en ;
	sh:targetClass indicators:ISO37120ClauseTenPointThree ;
	.

indicators:ISO37120ClauseTenPointTwo
	a
		owl:Class ,
		sh:NodeShape
		;
	rdfs:subClassOf indicators:GovernanceIndicator ;
	rdfs:label "ISO37120ClauseTenPointTwo"@en ;
	rdfs:comment "ISO 37120:2018 Clause 10.2 - Number of convictions for corruption and/or bribery by city officials per 100 000 population (supporting indicator)."@en ;
	sh:targetClass indicators:ISO37120ClauseTenPointTwo ;
	.

indicators:ISO37120ClauseThirteenPointFourPointFive
	a
		owl:Class ,
		sh:NodeShape
		;
	rdfs:subClassOf indicators:PopulationAndSocialConditionIndicator ;
	rdfs:label "ISO37120ClauseThirteenPointFourPointFive"@en ;
	rdfs:comment "ISO 37120:2018 Clause 13.4.5 - Percentage of city population that are non-citizens (profile indicator)."@en ;
	sh:targetClass indicators:ISO37120ClauseThirteenPointFourPointFive ;
	.

indicators:ISO37120ClauseThirteenPointFourPointFour
	a
		owl:Class ,
		sh:NodeShape
		;
	rdfs:subClassOf indicators:PopulationAndSocialConditionIndicator ;
	rdfs:label "ISO37120ClauseThirteenPointFourPointFour"@en ;
	rdfs:comment "ISO 37120:2018 Clause 13.4.4 - Percentage of population that are new immigrants (profile indicator)."@en ;
	sh:targetClass indicators:ISO37120ClauseThirteenPointFourPointFour ;
	.

indicators:ISO37120ClauseThirteenPointFourPointOne
	a
		owl:Class ,
		sh:NodeShape
		;
	rdfs:subClassOf indicators:PopulationAndSocialConditionIndicator ;
	rdfs:label "ISO37120ClauseThirteenPointFourPointOne"@en ;
	rdfs:comment "ISO 37120:2018 Clause 13.4.1 - Annual population change (profile indicator)."@en ;
	sh:targetClass indicators:ISO37120ClauseThirteenPointFourPointOne ;
	.

indicators:ISO37120ClauseThirteenPointFourPointSix
	a
		owl:Class ,
		sh:NodeShape
		;
	rdfs:subClassOf indicators:PopulationAndSocialConditionIndicator ;
	rdfs:label "ISO37120ClauseThirteenPointFourPointSix"@en ;
	rdfs:comment "ISO 37120:2018 Clause 13.4.6 - Number of university students per 100 000 population (profile indicator)."@en ;
	sh:targetClass indicators:ISO37120ClauseThirteenPointFourPointSix ;
	.

indicators:ISO37120ClauseThirteenPointFourPointThree
	a
		owl:Class ,
		sh:NodeShape
		;
	rdfs:subClassOf indicators:PopulationAndSocialConditionIndicator ;
	rdfs:label "ISO37120ClauseThirteenPointFourPointThree"@en ;
	rdfs:comment "ISO 37120:2018 Clause 13.4.3 - Population demographics (profile indicator)."@en ;
	sh:targetClass indicators:ISO37120ClauseThirteenPointFourPointThree ;
	.

indicators:ISO37120ClauseThirteenPointFourPointTwo
	a
		owl:Class ,
		sh:NodeShape
		;
	rdfs:subClassOf indicators:PopulationAndSocialConditionIndicator ;
	rdfs:label "ISO37120ClauseThirteenPointFourPointTwo"@en ;
	rdfs:comment "ISO 37120:2018 Clause 13.4.2 - Percentage of population that are foreign born (profile indicator)."@en ;
	sh:targetClass indicators:ISO37120ClauseThirteenPointFourPointTwo ;
	.

indicators:ISO37120ClauseThirteenPointOne
	a
		owl:Class ,
		sh:NodeShape
		;
	rdfs:subClassOf indicators:PopulationAndSocialConditionIndicator ;
	rdfs:label "ISO37120ClauseThirteenPointOne"@en ;
	rdfs:comment "ISO 37120:2018 Clause 13.1 - Percentage of city population living below the international poverty line (core indicator)."@en ;
	sh:targetClass indicators:ISO37120ClauseThirteenPointOne ;
	.

indicators:ISO37120ClauseThirteenPointThree
	a
		owl:Class ,
		sh:NodeShape
		;
	rdfs:subClassOf indicators:PopulationAndSocialConditionIndicator ;
	rdfs:label "ISO37120ClauseThirteenPointThree"@en ;
	rdfs:comment "ISO 37120:2018 Clause 13.3 - Gini coefficient of inequality (supporting indicator)."@en ;
	sh:targetClass indicators:ISO37120ClauseThirteenPointThree ;
	.

indicators:ISO37120ClauseThirteenPointTwo
	a
		owl:Class ,
		sh:NodeShape
		;
	rdfs:subClassOf indicators:PopulationAndSocialConditionIndicator ;
	rdfs:label "ISO37120ClauseThirteenPointTwo"@en ;
	rdfs:comment "ISO 37120:2018 Clause 13.2 - Percentage of city population living below the national poverty line (supporting indicator)."@en ;
	sh:targetClass indicators:ISO37120ClauseThirteenPointTwo ;
	.

indicators:ISO37120ClauseTwelvePointFivePointFive
	a
		owl:Class ,
		sh:NodeShape
		;
	rdfs:subClassOf indicators:HousingIndicator ;
	rdfs:label "ISO37120ClauseTwelvePointFivePointFive"@en ;
	rdfs:comment "ISO 37120:2018 Clause 12.5.5 - Secondary residence rate (profile indicator)."@en ;
	sh:targetClass indicators:ISO37120ClauseTwelvePointFivePointFive ;
	.

indicators:ISO37120ClauseTwelvePointFivePointFour
	a
		owl:Class ,
		sh:NodeShape
		;
	rdfs:subClassOf indicators:HousingIndicator ;
	rdfs:label "ISO37120ClauseTwelvePointFivePointFour"@en ;
	rdfs:comment "ISO 37120:2018 Clause 12.5.4 - Living space (square metres) per person (profile indicator)."@en-gb ;
	sh:targetClass indicators:ISO37120ClauseTwelvePointFivePointFour ;
	.

indicators:ISO37120ClauseTwelvePointFivePointOne
	a
		owl:Class ,
		sh:NodeShape
		;
	rdfs:subClassOf indicators:HousingIndicator ;
	rdfs:label "ISO37120ClauseTwelvePointFivePointOne"@en ;
	rdfs:comment "ISO 37120:2018 Clause 12.5.1 - Total number of households (profile indicator)."@en ;
	sh:targetClass indicators:ISO37120ClauseTwelvePointFivePointOne ;
	.

indicators:ISO37120ClauseTwelvePointFivePointSix
	a
		owl:Class ,
		sh:NodeShape
		;
	rdfs:subClassOf indicators:HousingIndicator ;
	rdfs:label "ISO37120ClauseTwelvePointFivePointSix"@en ;
	rdfs:comment "ISO 37120:2018 Clause 12.5.6 - Residential rental dwelling units as a percentage of total dwelling units (profile indicator)."@en ;
	sh:targetClass indicators:ISO37120ClauseTwelvePointFivePointSix ;
	.

indicators:ISO37120ClauseTwelvePointFivePointThree
	a
		owl:Class ,
		sh:NodeShape
		;
	rdfs:subClassOf indicators:HousingIndicator ;
	rdfs:label "ISO37120ClauseTwelvePointFivePointThree"@en ;
	rdfs:comment "ISO 37120:2018 Clause 12.5.3 - Vacancy rate (residential) (profile indicator)."@en ;
	sh:targetClass indicators:ISO37120ClauseTwelvePointFivePointThree ;
	.

indicators:ISO37120ClauseTwelvePointFivePointTwo
	a
		owl:Class ,
		sh:NodeShape
		;
	rdfs:subClassOf indicators:HousingIndicator ;
	rdfs:label "ISO37120ClauseTwelvePointFivePointTwo"@en ;
	rdfs:comment "ISO 37120:2018 Clause 12.5.2 - Persons per unit (profile indicator)."@en ;
	sh:targetClass indicators:ISO37120ClauseTwelvePointFivePointTwo ;
	.

indicators:ISO37120ClauseTwelvePointFour
	a
		owl:Class ,
		sh:NodeShape
		;
	rdfs:subClassOf indicators:HousingIndicator ;
	rdfs:label "ISO37120ClauseTwelvePointFour"@en ;
	rdfs:comment "ISO 37120:2018 Clause 12.4 - Percentage of households that exist without registered legal titles (supporting indicator)."@en ;
	sh:targetClass indicators:ISO37120ClauseTwelvePointFour ;
	.

indicators:ISO37120ClauseTwelvePointOne
	a
		owl:Class ,
		sh:NodeShape
		;
	rdfs:subClassOf indicators:HousingIndicator ;
	rdfs:label "ISO37120ClauseTwelvePointOne"@en ;
	rdfs:comment "ISO 37120:2018 Clause 12.1 - Percentage of city population living in inadequate housing (core indicator)."@en ;
	sh:targetClass indicators:ISO37120ClauseTwelvePointOne ;
	.

indicators:ISO37120ClauseTwelvePointThree
	a
		owl:Class ,
		sh:NodeShape
		;
	rdfs:subClassOf indicators:HousingIndicator ;
	rdfs:label "ISO37120ClauseTwelvePointThree"@en ;
	rdfs:comment "ISO 37120:2018 Clause 12.3 - Number of homeless per 100 000 population (supporting indicator)."@en ;
	sh:targetClass indicators:ISO37120ClauseTwelvePointThree ;
	.

indicators:ISO37120ClauseTwelvePointTwo
	a
		owl:Class ,
		sh:NodeShape
		;
	rdfs:subClassOf indicators:HousingIndicator ;
	rdfs:label "ISO37120ClauseTwelvePointTwo"@en ;
	rdfs:comment "ISO 37120:2018 Clause 12.2 - Percentage of population living in affordable housing (core indicator)."@en ;
	sh:targetClass indicators:ISO37120ClauseTwelvePointTwo ;
	.

indicators:ISO37120ClauseTwentyOnePointFivePointOne
	a
		owl:Class ,
		sh:NodeShape
		;
	rdfs:subClassOf indicators:UrbanPlanningIndicator ;
	rdfs:label "ISO37120ClauseTwentyOnePointFivePointOne"@en ;
	rdfs:comment "ISO 37120:2018 Clause 21.5.1 - Population density (per square kilometre) (profile indicator)."@en ;
	sh:targetClass indicators:ISO37120ClauseTwentyOnePointFivePointOne ;
	.

indicators:ISO37120ClauseTwentyOnePointFivePointThree
	a
		owl:Class ,
		sh:NodeShape
		;
	rdfs:subClassOf indicators:UrbanPlanningIndicator ;
	rdfs:label "ISO37120ClauseTwentyOnePointFivePointThree"@en ;
	rdfs:comment "ISO 37120:2018 Clause 21.5.3 - Built-up density (profile indicator)."@en ;
	sh:targetClass indicators:ISO37120ClauseTwentyOnePointFivePointThree ;
	.

indicators:ISO37120ClauseTwentyOnePointFivePointTwo
	a
		owl:Class ,
		sh:NodeShape
		;
	rdfs:subClassOf indicators:UrbanPlanningIndicator ;
	rdfs:label "ISO37120ClauseTwentyOnePointFivePointTwo"@en ;
	rdfs:comment "ISO 37120:2018 Clause 21.5.2 - Number of trees per 100 000 population (profile indicator)."@en ;
	sh:targetClass indicators:ISO37120ClauseTwentyOnePointFivePointTwo ;
	.

indicators:ISO37120ClauseTwentyOnePointFour
	a
		owl:Class ,
		sh:NodeShape
		;
	rdfs:subClassOf indicators:UrbanPlanningIndicator ;
	rdfs:label "ISO37120ClauseTwentyOnePointFour"@en ;
	rdfs:comment "ISO 37120:2018 Clause 21.4 - Basic service proximity (supporting indicator)."@en ;
	sh:targetClass indicators:ISO37120ClauseTwentyOnePointFour ;
	.

indicators:ISO37120ClauseTwentyOnePointOne
	a
		owl:Class ,
		sh:NodeShape
		;
	rdfs:subClassOf indicators:UrbanPlanningIndicator ;
	rdfs:label "ISO37120ClauseTwentyOnePointOne"@en ;
	rdfs:comment "ISO 37120:2018 Clause 21.1 - Green area (hectares) per 100 000 population (core indicator)."@en ;
	sh:targetClass indicators:ISO37120ClauseTwentyOnePointOne ;
	.

indicators:ISO37120ClauseTwentyOnePointThree
	a
		owl:Class ,
		sh:NodeShape
		;
	rdfs:subClassOf indicators:UrbanPlanningIndicator ;
	rdfs:label "ISO37120ClauseTwentyOnePointThree"@en ;
	rdfs:comment "ISO 37120:2018 Clause 21.3 - Jobs–housing ratio (supporting indicator)."@en ;
	sh:targetClass indicators:ISO37120ClauseTwentyOnePointThree ;
	.

indicators:ISO37120ClauseTwentyOnePointTwo
	a
		owl:Class ,
		sh:NodeShape
		;
	rdfs:subClassOf indicators:UrbanPlanningIndicator ;
	rdfs:label "ISO37120ClauseTwentyOnePointTwo"@en ;
	rdfs:comment "ISO 37120:2018 Clause 21.2 - Areal size of informal settlements as a percentage of city area (supporting indicator)."@en ;
	sh:targetClass indicators:ISO37120ClauseTwentyOnePointTwo ;
	.

indicators:ISO37120ClauseTwentyPointFour
	a
		owl:Class ,
		sh:NodeShape
		;
	rdfs:subClassOf indicators:UrbanLocalAgricultureAndFoodSecurityIndicator ;
	rdfs:label "ISO37120ClauseTwentyPointFour"@en ;
	rdfs:comment "ISO 37120:2018 Clause 20.4 - 20.4	Percentage of city population that is overweight or obese — Body Mass Index (BMI) (supporting indicator)."@en ;
	sh:targetClass indicators:ISO37120ClauseTwentyPointFour ;
	.

indicators:ISO37120ClauseTwentyPointOne
	a
		owl:Class ,
		sh:NodeShape
		;
	rdfs:subClassOf indicators:UrbanLocalAgricultureAndFoodSecurityIndicator ;
	rdfs:label "ISO37120ClauseTwentyPointOne"@en ;
	rdfs:comment "ISO 37120:2018 Clause 20.1 - Total urban agricultural area per 100 000 population (core indicator)."@en ;
	sh:targetClass indicators:ISO37120ClauseTwentyPointOne ;
	.

indicators:ISO37120ClauseTwentyPointThree
	a
		owl:Class ,
		sh:NodeShape
		;
	rdfs:subClassOf indicators:UrbanLocalAgricultureAndFoodSecurityIndicator ;
	rdfs:label "ISO37120ClauseTwentyPointThree"@en ;
	rdfs:comment "ISO 37120:2018 Clause 20.3 - Percentage of city population undernourished (supporting indicator)."@en ;
	sh:targetClass indicators:ISO37120ClauseTwentyPointThree ;
	.

indicators:ISO37120ClauseTwentyPointTwo
	a
		owl:Class ,
		sh:NodeShape
		;
	rdfs:subClassOf indicators:UrbanLocalAgricultureAndFoodSecurityIndicator ;
	rdfs:label "ISO37120ClauseTwentyPointTwo"@en ;
	rdfs:comment "ISO 37120:2018 Clause 20.2 - Amount of food produced locally as a percentage of total food supplied to the city (supporting indicator)."@en ;
	sh:targetClass indicators:ISO37120ClauseTwentyPointTwo ;
	.

indicators:ISO37120ClauseTwentyThreePointFive
	a
		owl:Class ,
		sh:NodeShape
		;
	rdfs:subClassOf indicators:WaterIndicator ;
	rdfs:label "ISO37120ClauseTwentyThreePointFive"@en ;
	rdfs:comment "ISO 37120:2018 Clause 23.5 - Total water consumption per capita (litres/day) (supporting indicator)."@en-gb ;
	sh:targetClass indicators:ISO37120ClauseTwentyThreePointFive ;
	.

indicators:ISO37120ClauseTwentyThreePointFour
	a
		owl:Class ,
		sh:NodeShape
		;
	rdfs:subClassOf indicators:WaterIndicator ;
	rdfs:label "ISO37120ClauseTwentyThreePointFour"@en ;
	rdfs:comment "ISO 37120:2018 Clause 23.4 - Compliance rate of drinking water quality (core indicator)."@en ;
	sh:targetClass indicators:ISO37120ClauseTwentyThreePointFour ;
	.

indicators:ISO37120ClauseTwentyThreePointOne
	a
		owl:Class ,
		sh:NodeShape
		;
	rdfs:subClassOf indicators:WaterIndicator ;
	rdfs:label "ISO37120ClauseTwentyThreePointOne"@en ;
	rdfs:comment "ISO 37120:2018 Clause 23.1 - Percentage of city population with potable water supply service (core indicator)."@en ;
	sh:targetClass indicators:ISO37120ClauseTwentyThreePointOne ;
	.

indicators:ISO37120ClauseTwentyThreePointSeven
	a
		owl:Class ,
		sh:NodeShape
		;
	rdfs:subClassOf indicators:WaterIndicator ;
	rdfs:label "ISO37120ClauseTwentyThreePointSeven"@en ;
	rdfs:comment "ISO 37120:2018 Clause 23.7 - Percentage of water loss (unaccounted for water) (supporting indicator)."@en ;
	sh:targetClass indicators:ISO37120ClauseTwentyThreePointSeven ;
	.

indicators:ISO37120ClauseTwentyThreePointSix
	a
		owl:Class ,
		sh:NodeShape
		;
	rdfs:subClassOf indicators:WaterIndicator ;
	rdfs:label "ISO37120ClauseTwentyThreePointSix"@en ;
	rdfs:comment "ISO 37120:2018 Clause 23.6 - Average annual hours of water service interruptions per household (supporting indicator)."@en ;
	sh:targetClass indicators:ISO37120ClauseTwentyThreePointSix ;
	.

indicators:ISO37120ClauseTwentyThreePointThree
	a
		owl:Class ,
		sh:NodeShape
		;
	rdfs:subClassOf indicators:WaterIndicator ;
	rdfs:label "ISO37120ClauseTwentyThreePointThree"@en ;
	rdfs:comment "ISO 37120:2018 Clause 23.3 - Total domestic water consumption per capita (litres/day) (core indicator)."@en-gb ;
	sh:targetClass indicators:ISO37120ClauseTwentyThreePointThree ;
	.

indicators:ISO37120ClauseTwentyThreePointTwo
	a
		owl:Class ,
		sh:NodeShape
		;
	rdfs:subClassOf indicators:WaterIndicator ;
	rdfs:label "ISO37120ClauseTwentyThreePointTwo"@en ;
	rdfs:comment "ISO 37120:2018 Clause 23.2 - Percentage of city population with sustainable access to an improved water source (core indicator)."@en ;
	sh:targetClass indicators:ISO37120ClauseTwentyThreePointTwo ;
	.

indicators:ISO37120ClauseTwentyTwoPointFour
	a
		owl:Class ,
		sh:NodeShape
		;
	rdfs:subClassOf indicators:WastewaterIndicator ;
	rdfs:label "ISO37120ClauseTwentyTwoPointFour"@en ;
	rdfs:comment "ISO 37120:2018 Clause 22.4 - Compliance rate of wastewater treatment (supporting indicator)."@en ;
	sh:targetClass indicators:ISO37120ClauseTwentyTwoPointFour ;
	.

indicators:ISO37120ClauseTwentyTwoPointOne
	a
		owl:Class ,
		sh:NodeShape
		;
	rdfs:subClassOf indicators:WastewaterIndicator ;
	rdfs:label "ISO37120ClauseTwentyTwoPointOne"@en ;
	rdfs:comment "ISO 37120:2018 Clause 22.1 - Percentage of city population served by wastewater collection (core indicator)."@en ;
	sh:targetClass indicators:ISO37120ClauseTwentyTwoPointOne ;
	.

indicators:ISO37120ClauseTwentyTwoPointThree
	a
		owl:Class ,
		sh:NodeShape
		;
	rdfs:subClassOf indicators:WastewaterIndicator ;
	rdfs:label "ISO37120ClauseTwentyTwoPointThree"@en ;
	rdfs:comment "ISO 37120:2018 Clause 22.3 - Percentage of population with access to improved sanitation (core indicator)."@en ;
	sh:targetClass indicators:ISO37120ClauseTwentyTwoPointThree ;
	.

indicators:ISO37120ClauseTwentyTwoPointTwo
	a
		owl:Class ,
		sh:NodeShape
		;
	rdfs:subClassOf indicators:WastewaterIndicator ;
	rdfs:label "ISO37120ClauseTwentyTwoPointTwo"@en ;
	rdfs:comment "ISO 37120:2018 Clause 22.2 - Percentage of city’s wastewater receiving centralized treatment (core indicator)."@en ;
	sh:targetClass indicators:ISO37120ClauseTwentyTwoPointTwo ;
	.

indicators:ISO37122ClauseEightPointOne
	a
		owl:Class ,
		sh:NodeShape
		;
	rdfs:subClassOf indicators:EnvironmentAndClimateChangeIndicator ;
	rdfs:label "ISO37122ClauseEightPointOne"@en ;
	rdfs:comment "ISO 37122:2019 Clause 8.1 - Percentage of buildings built or refurbished within the last 5 years in conformity with green building principles."@en ;
	sh:targetClass indicators:ISO37122ClauseEightPointOne ;
	.

indicators:ISO37122ClauseEightPointThree
	a
		owl:Class ,
		sh:NodeShape
		;
	rdfs:subClassOf indicators:EnvironmentAndClimateChangeIndicator ;
	rdfs:label "ISO37122ClauseEightPointThree"@en ;
	rdfs:comment "ISO 37122:2019 Clause 8.3 - Percentage of public buildings equipped for monitoring indoor air quality."@en ;
	sh:targetClass indicators:ISO37122ClauseEightPointThree ;
	.

indicators:ISO37122ClauseEightPointTwo
	a
		owl:Class ,
		sh:NodeShape
		;
	rdfs:subClassOf indicators:EnvironmentAndClimateChangeIndicator ;
	rdfs:label "ISO37122ClauseEightPointTwo"@en ;
	rdfs:comment "ISO 37122:2019 Clause 8.2 - Number of real-time remote air quality monitoring stations per square kilometre (km2)."@en-gb ;
	sh:targetClass indicators:ISO37122ClauseEightPointTwo ;
	.

indicators:ISO37122ClauseEighteenPointOne
	a
		owl:Class ,
		sh:NodeShape
		;
	rdfs:subClassOf indicators:TelecommunicationIndicator ;
	rdfs:label "ISO37122ClauseEighteenPointOne"@en ;
	rdfs:comment "ISO 37122:2019 Clause 18.1 - Percentage of the city population with access to sufficiently fast broadband."@en ;
	sh:targetClass indicators:ISO37122ClauseEighteenPointOne ;
	.

indicators:ISO37122ClauseEighteenPointThree
	a
		owl:Class ,
		sh:NodeShape
		;
	rdfs:subClassOf indicators:TelecommunicationIndicator ;
	rdfs:label "ISO37122ClauseEighteenPointThree"@en ;
	rdfs:comment "ISO 37122:2019 Clause 18.3 - Percentage of the city area covered by municipally provided Internet connectivity."@en ;
	sh:targetClass indicators:ISO37122ClauseEighteenPointThree ;
	.

indicators:ISO37122ClauseEighteenPointTwo
	a
		owl:Class ,
		sh:NodeShape
		;
	rdfs:subClassOf indicators:TelecommunicationIndicator ;
	rdfs:label "ISO37122ClauseEighteenPointTwo"@en ;
	rdfs:comment "ISO 37122:2019 Clause 18.2 - Percentage of city area under a white zone/dead spot/not covered by telecommunication connectivity."@en ;
	sh:targetClass indicators:ISO37122ClauseEighteenPointTwo ;
	.

indicators:ISO37122ClauseElevenPointOne
	a
		owl:Class ,
		sh:NodeShape
		;
	rdfs:subClassOf indicators:HealthIndicator ;
	rdfs:label "ISO37122ClauseElevenPointOne"@en ;
	rdfs:comment "ISO 37122:2019 Clause 11.1 - Percentage of the city’s population with an online unified health file accessible to health care providers."@en ;
	sh:targetClass indicators:ISO37122ClauseElevenPointOne ;
	.

indicators:ISO37122ClauseElevenPointThree
	a
		owl:Class ,
		sh:NodeShape
		;
	rdfs:subClassOf indicators:HealthIndicator ;
	rdfs:label "ISO37122ClauseElevenPointThree"@en ;
	rdfs:comment "ISO 37122:2019 Clause 11.3 - Percentage of the city population with access to real-time public alert systems for air and water quality advisories."@en ;
	sh:targetClass indicators:ISO37122ClauseElevenPointThree ;
	.

indicators:ISO37122ClauseElevenPointTwo
	a
		owl:Class ,
		sh:NodeShape
		;
	rdfs:subClassOf indicators:HealthIndicator ;
	rdfs:label "ISO37122ClauseElevenPointTwo"@en ;
	rdfs:comment "ISO 37122:2019 Clause 11.2 - Annual number of medical appointments conducted remotely per 100 000 population."@en ;
	sh:targetClass indicators:ISO37122ClauseElevenPointTwo ;
	.

indicators:ISO37122ClauseFifteenPointOne
	a
		owl:Class ,
		sh:NodeShape
		;
	rdfs:subClassOf indicators:SafetyIndicator ;
	rdfs:label "ISO37122ClauseFifteenPointOne"@en ;
	rdfs:comment "ISO 37122:2019 Clause 15.1 - Percentage of the city area covered by digital surveillance cameras."@en ;
	sh:targetClass indicators:ISO37122ClauseFifteenPointOne ;
	.

indicators:ISO37122ClauseFivePointFour
	a
		owl:Class ,
		sh:NodeShape
		;
	rdfs:subClassOf indicators:EconomyIndicator ;
	rdfs:label "ISO37122ClauseFivePointFour"@en ;
	rdfs:comment "ISO 37122:2019 Clause 5.4 - Percentage of the labour force employed in occupations in the education and research and development sectors."@en-gb ;
	sh:targetClass indicators:ISO37122ClauseFivePointFour ;
	.

indicators:ISO37122ClauseFivePointOne
	a
		owl:Class ,
		sh:NodeShape
		;
	rdfs:subClassOf indicators:EconomyIndicator ;
	rdfs:label "ISO37122ClauseFivePointOne"@en ;
	rdfs:comment "ISO 37122:2019 Clause 5.1 - Percentage of service contracts providing city services which contain an open data policy."@en ;
	sh:targetClass indicators:ISO37122ClauseFivePointOne ;
	.

indicators:ISO37122ClauseFivePointThree
	a
		owl:Class ,
		sh:NodeShape
		;
	rdfs:subClassOf indicators:EconomyIndicator ;
	rdfs:label "ISO37122ClauseFivePointThree"@en ;
	rdfs:comment "ISO 37122:2019 Clause 5.3 - Percentage of the labour force employed in occupations in the information and communications technology (ICT) sector."@en-gb ;
	sh:targetClass indicators:ISO37122ClauseFivePointThree ;
	.

indicators:ISO37122ClauseFivePointTwo
	a
		owl:Class ,
		sh:NodeShape
		;
	rdfs:subClassOf indicators:EconomyIndicator ;
	rdfs:label "ISO37122ClauseFivePointTwo"@en ;
	rdfs:comment "ISO 37122:2019 Clause 5.2 - Survival rate of new businesses per 100 000 population."@en ;
	sh:targetClass indicators:ISO37122ClauseFivePointTwo ;
	.

indicators:ISO37122ClauseFourteenPointOne
	a
		owl:Class ,
		sh:NodeShape
		;
	rdfs:subClassOf indicators:RecreationIndicator ;
	rdfs:label "ISO37122ClauseFourteenPointOne"@en ;
	rdfs:comment "ISO 37122:2019 Clause 14.1 - Percentage of public recreation services that can be booked online."@en ;
	sh:targetClass indicators:ISO37122ClauseFourteenPointOne ;
	.

indicators:ISO37122ClauseNinePointOne
	a
		owl:Class ,
		sh:NodeShape
		;
	rdfs:subClassOf indicators:FinanceIndicator ;
	rdfs:label "ISO37122ClauseNinePointOne"@en ;
	rdfs:comment "ISO 37122:2019 Clause 9.1 - Annual amount of revenues collected from the sharing economy as a percentage of own-source revenue."@en ;
	sh:targetClass indicators:ISO37122ClauseNinePointOne ;
	.

indicators:ISO37122ClauseNinePointTwo
	a
		owl:Class ,
		sh:NodeShape
		;
	rdfs:subClassOf indicators:FinanceIndicator ;
	rdfs:label "ISO37122ClauseNinePointTwo"@en ;
	rdfs:comment "ISO 37122:2019 Clause 9.2 - Percentage of payments to the city that are paid electronically based on electronic invoices."@en ;
	sh:targetClass indicators:ISO37122ClauseNinePointTwo ;
	.

indicators:ISO37122ClauseNineteenPointEight
	a
		owl:Class ,
		sh:NodeShape
		;
	rdfs:subClassOf indicators:TransportationIndicator ;
	rdfs:label "ISO37122ClauseNineteenPointEight"@en ;
	rdfs:comment "ISO 37122:2019 Clause 19.8 - Percentage of public parking spaces equipped with real-time availability systems."@en ;
	sh:targetClass indicators:ISO37122ClauseNineteenPointEight ;
	.

indicators:ISO37122ClauseNineteenPointEleven
	a
		owl:Class ,
		sh:NodeShape
		;
	rdfs:subClassOf indicators:TransportationIndicator ;
	rdfs:label "ISO37122ClauseNineteenPointEleven"@en ;
	rdfs:comment "ISO 37122:2019 Clause 19.11 - Percentage of vehicles registered in the city that are autonomous vehicles."@en ;
	sh:targetClass indicators:ISO37122ClauseNineteenPointEleven ;
	.

indicators:ISO37122ClauseNineteenPointFive
	a
		owl:Class ,
		sh:NodeShape
		;
	rdfs:subClassOf indicators:TransportationIndicator ;
	rdfs:label "ISO37122ClauseNineteenPointFive"@en ;
	rdfs:comment "ISO 37122:2019 Clause 19.5 - Percentage of public transport lines equipped with a publicly accessible real-time system."@en ;
	sh:targetClass indicators:ISO37122ClauseNineteenPointFive ;
	.

indicators:ISO37122ClauseNineteenPointFour
	a
		owl:Class ,
		sh:NodeShape
		;
	rdfs:subClassOf indicators:TransportationIndicator ;
	rdfs:label "ISO37122ClauseNineteenPointFour"@en ;
	rdfs:comment "ISO 37122:2019 Clause 19.4 - Number of bicycles available through municipally provided bicycle-sharing services per 100 000 population."@en ;
	sh:targetClass indicators:ISO37122ClauseNineteenPointFour ;
	.

indicators:ISO37122ClauseNineteenPointFourteen
	a
		owl:Class ,
		sh:NodeShape
		;
	rdfs:subClassOf indicators:TransportationIndicator ;
	rdfs:label "ISO37122ClauseNineteenPointFourteen"@en ;
	rdfs:comment "ISO 37122:2019 Clause 19.14 - Percentage of the city’s bus fleet that is motor-driven."@en ;
	sh:targetClass indicators:ISO37122ClauseNineteenPointFourteen ;
	.

indicators:ISO37122ClauseNineteenPointNine
	a
		owl:Class ,
		sh:NodeShape
		;
	rdfs:subClassOf indicators:TransportationIndicator ;
	rdfs:label "ISO37122ClauseNineteenPointNine"@en ;
	rdfs:comment "ISO 37122:2019 Clause 19.9 - Percentage of traffic lights that are intelligent/smart."@en ;
	sh:targetClass indicators:ISO37122ClauseNineteenPointNine ;
	.

indicators:ISO37122ClauseNineteenPointOne
	a
		owl:Class ,
		sh:NodeShape
		;
	rdfs:subClassOf indicators:TransportationIndicator ;
	rdfs:label "ISO37122ClauseNineteenPointOne"@en ;
	rdfs:comment "ISO 37122:2019 Clause 19.1 - Percentage of city streets and thoroughfares covered by real-time online traffic alerts and information."@en ;
	sh:targetClass indicators:ISO37122ClauseNineteenPointOne ;
	.

indicators:ISO37122ClauseNineteenPointSeven
	a
		owl:Class ,
		sh:NodeShape
		;
	rdfs:subClassOf indicators:TransportationIndicator ;
	rdfs:label "ISO37122ClauseNineteenPointSeven"@en ;
	rdfs:comment "ISO 37122:2019 Clause 19.7 - Percentage of public parking spaces equipped with e-payment systems."@en ;
	sh:targetClass indicators:ISO37122ClauseNineteenPointSeven ;
	.

indicators:ISO37122ClauseNineteenPointSix
	a
		owl:Class ,
		sh:NodeShape
		;
	rdfs:subClassOf indicators:TransportationIndicator ;
	rdfs:label "ISO37122ClauseNineteenPointSix"@en ;
	rdfs:comment "ISO 37122:2019 Clause 19.6 - Percentage of the city’s public transport services covered by a unified payment system."@en ;
	sh:targetClass indicators:ISO37122ClauseNineteenPointSix ;
	.

indicators:ISO37122ClauseNineteenPointTen
	a
		owl:Class ,
		sh:NodeShape
		;
	rdfs:subClassOf indicators:TransportationIndicator ;
	rdfs:label "ISO37122ClauseNineteenPointTen"@en ;
	rdfs:comment "ISO 37122:2019 Clause 19.10 - City area mapped by real-time interactive street maps as a percentage of the city’s total land area."@en ;
	sh:targetClass indicators:ISO37122ClauseNineteenPointTen ;
	.

indicators:ISO37122ClauseNineteenPointThirteen
	a
		owl:Class ,
		sh:NodeShape
		;
	rdfs:subClassOf indicators:TransportationIndicator ;
	rdfs:label "ISO37122ClauseNineteenPointThirteen"@en ;
	rdfs:comment "ISO 37122:2019 Clause 19.13 - Percentage of roads conforming with autonomous driving systems."@en ;
	sh:targetClass indicators:ISO37122ClauseNineteenPointThirteen ;
	.

indicators:ISO37122ClauseNineteenPointThree
	a
		owl:Class ,
		sh:NodeShape
		;
	rdfs:subClassOf indicators:TransportationIndicator ;
	rdfs:label "ISO37122ClauseNineteenPointThree"@en ;
	rdfs:comment "ISO 37122:2019 Clause 19.3 - Percentage of vehicles registered in the city that are low-emission vehicles."@en ;
	sh:targetClass indicators:ISO37122ClauseNineteenPointThree ;
	.

indicators:ISO37122ClauseNineteenPointTwelve
	a
		owl:Class ,
		sh:NodeShape
		;
	rdfs:subClassOf indicators:TransportationIndicator ;
	rdfs:label "ISO37122ClauseNineteenPointTwelve"@en ;
	rdfs:comment "ISO 37122:2019 Clause 19.12 - Percentage of public transport routes with municipally provided and/or managed Internet connectivity for commuters."@en ;
	sh:targetClass indicators:ISO37122ClauseNineteenPointTwelve ;
	.

indicators:ISO37122ClauseNineteenPointTwo
	a
		owl:Class ,
		sh:NodeShape
		;
	rdfs:subClassOf indicators:TransportationIndicator ;
	rdfs:label "ISO37122ClauseNineteenPointTwo"@en ;
	rdfs:comment "ISO 37122:2019 Clause 19.2 - Number of users of sharing economy transportation per 100 000 population."@en ;
	sh:targetClass indicators:ISO37122ClauseNineteenPointTwo ;
	.

indicators:ISO37122ClauseSevenPointEight
	a
		owl:Class ,
		sh:NodeShape
		;
	rdfs:subClassOf indicators:EnergyIndicator ;
	rdfs:label "ISO37122ClauseSevenPointEight"@en ;
	rdfs:comment "ISO 37122:2019 Clause 7.8 - Percentage of public buildings requiring renovation/refurbishment."@en ;
	sh:targetClass indicators:ISO37122ClauseSevenPointEight ;
	.

indicators:ISO37122ClauseSevenPointFive
	a
		owl:Class ,
		sh:NodeShape
		;
	rdfs:subClassOf indicators:EnergyIndicator ;
	rdfs:label "ISO37122ClauseSevenPointFive"@en ;
	rdfs:comment "ISO 37122:2019 Clause 7.5 - Storage capacity of the city’s energy grid per total city energy consumption."@en ;
	sh:targetClass indicators:ISO37122ClauseSevenPointFive ;
	.

indicators:ISO37122ClauseSevenPointFour
	a
		owl:Class ,
		sh:NodeShape
		;
	rdfs:subClassOf indicators:EnergyIndicator ;
	rdfs:label "ISO37122ClauseSevenPointFour"@en ;
	rdfs:comment "ISO 37122:2019 Clause 7.4 - Percentage of the city’s electricity that is produced using decentralised electricity production systems."@en-gb ;
	sh:targetClass indicators:ISO37122ClauseSevenPointFour ;
	.

indicators:ISO37122ClauseSevenPointNine
	a
		owl:Class ,
		sh:NodeShape
		;
	rdfs:subClassOf indicators:EnergyIndicator ;
	rdfs:label "ISO37122ClauseSevenPointNine"@en ;
	rdfs:comment "ISO 37122:2019 Clause 7.9 - Percentage of buildings in the city with smart energy meters."@en ;
	sh:targetClass indicators:ISO37122ClauseSevenPointNine ;
	.

indicators:ISO37122ClauseSevenPointOne
	a
		owl:Class ,
		sh:NodeShape
		;
	rdfs:subClassOf indicators:EnergyIndicator ;
	rdfs:label "ISO37122ClauseSevenPointOne"@en ;
	rdfs:comment "ISO 37122:2019 Clause 7.1 - Percentage of electrical and thermal energy produced from wastewater treatment, solid waste and other liquid waste treatment and other waste heat resources, as a share of the city’s total energy mix for a given year."@en ;
	sh:targetClass indicators:ISO37122ClauseSevenPointOne ;
	.

indicators:ISO37122ClauseSevenPointSeven
	a
		owl:Class ,
		sh:NodeShape
		;
	rdfs:subClassOf indicators:EnergyIndicator ;
	rdfs:label "ISO37122ClauseSevenPointSeven"@en ;
	rdfs:comment "ISO 37122:2019 Clause 7.7 - Percentage of street lighting that has been refurbished and newly installed."@en ;
	sh:targetClass indicators:ISO37122ClauseSevenPointSeven ;
	.

indicators:ISO37122ClauseSevenPointSix
	a
		owl:Class ,
		sh:NodeShape
		;
	rdfs:subClassOf indicators:EnergyIndicator ;
	rdfs:label "ISO37122ClauseSevenPointSix"@en ;
	rdfs:comment "ISO 37122:2019 Clause 7.6 - Percentage of street lighting managed by a light performance management system."@en ;
	sh:targetClass indicators:ISO37122ClauseSevenPointSix ;
	.

indicators:ISO37122ClauseSevenPointTen
	a
		owl:Class ,
		sh:NodeShape
		;
	rdfs:subClassOf indicators:EnergyIndicator ;
	rdfs:label "ISO37122ClauseSevenPointTen"@en ;
	rdfs:comment "ISO 37122:2019 Clause 7.10 - Number of electric vehicle charging stations per registered electric vehicle."@en ;
	sh:targetClass indicators:ISO37122ClauseSevenPointTen ;
	.

indicators:ISO37122ClauseSevenPointThree
	a
		owl:Class ,
		sh:NodeShape
		;
	rdfs:subClassOf indicators:EnergyIndicator ;
	rdfs:label "ISO37122ClauseSevenPointThree"@en ;
	rdfs:comment "ISO 37122:2019 Clause 7.3 - Electrical and thermal energy (GJ) produced from solid waste or other liquid waste treatment per capita per year."@en ;
	sh:targetClass indicators:ISO37122ClauseSevenPointThree ;
	.

indicators:ISO37122ClauseSevenPointTwo
	a
		owl:Class ,
		sh:NodeShape
		;
	rdfs:subClassOf indicators:EnergyIndicator ;
	rdfs:label "ISO37122ClauseSevenPointTwo"@en ;
	rdfs:comment "ISO 37122:2019 Clause 7.2 - Electrical and thermal energy (GJ) produced from wastewater treatment per capita per year."@en ;
	sh:targetClass indicators:ISO37122ClauseSevenPointTwo ;
	.

indicators:ISO37122ClauseSeventeenPointFour
	a
		owl:Class ,
		sh:NodeShape
		;
	rdfs:subClassOf indicators:SportAndCultureIndicator ;
	rdfs:label "ISO37122ClauseSeventeenPointFour"@en ;
	rdfs:comment "ISO 37122:2019 Clause 17.4 - Percentage of city population that are active public library users."@en ;
	sh:targetClass indicators:ISO37122ClauseSeventeenPointFour ;
	.

indicators:ISO37122ClauseSeventeenPointOne
	a
		owl:Class ,
		sh:NodeShape
		;
	rdfs:subClassOf indicators:SportAndCultureIndicator ;
	rdfs:label "ISO37122ClauseSeventeenPointOne"@en ;
	rdfs:comment "ISO 37122:2019 Clause 17.1 - Number of online bookings for cultural facilities per 100 000 population."@en ;
	sh:targetClass indicators:ISO37122ClauseSeventeenPointOne ;
	.

indicators:ISO37122ClauseSeventeenPointThree
	a
		owl:Class ,
		sh:NodeShape
		;
	rdfs:subClassOf indicators:SportAndCultureIndicator ;
	rdfs:label "ISO37122ClauseSeventeenPointThree"@en ;
	rdfs:comment "ISO 37122:2019 Clause 17.3 - Number of public library book and e-book titles per 100 000 population."@en ;
	sh:targetClass indicators:ISO37122ClauseSeventeenPointThree ;
	.

indicators:ISO37122ClauseSeventeenPointTwo
	a
		owl:Class ,
		sh:NodeShape
		;
	rdfs:subClassOf indicators:SportAndCultureIndicator ;
	rdfs:label "ISO37122ClauseSeventeenPointTwo"@en ;
	rdfs:comment "ISO 37122:2019 Clause 17.2 - Percentage of the city’s cultural records that have been digitised."@en-gb ;
	sh:targetClass indicators:ISO37122ClauseSeventeenPointTwo ;
	.

indicators:ISO37122ClauseSixPointOne
	a
		owl:Class ,
		sh:NodeShape
		;
	rdfs:subClassOf indicators:EducationIndicator ;
	rdfs:label "ISO37122ClauseSixPointOne"@en ;
	rdfs:comment "ISO 37122:2019 Clause 6.1 - Percentage of city population with professional proficiency in more than one language."@en ;
	sh:targetClass indicators:ISO37122ClauseSixPointOne ;
	.

indicators:ISO37122ClauseSixPointThree
	a
		owl:Class ,
		sh:NodeShape
		;
	rdfs:subClassOf indicators:EducationIndicator ;
	rdfs:label "ISO37122ClauseSixPointThree"@en ;
	rdfs:comment "ISO 37122:2019 Clause 6.3 - Number of science, technology, engineering and mathematics (STEM) higher education degrees per 100 000 population."@en ;
	sh:targetClass indicators:ISO37122ClauseSixPointThree ;
	.

indicators:ISO37122ClauseSixPointTwo
	a
		owl:Class ,
		sh:NodeShape
		;
	rdfs:subClassOf indicators:EducationIndicator ;
	rdfs:label "ISO37122ClauseSixPointTwo"@en ;
	rdfs:comment "ISO 37122:2019 Clause 6.2 - Number of computers, laptops, tablets or other digital learning devices available per 1 000 students."@en ;
	sh:targetClass indicators:ISO37122ClauseSixPointTwo ;
	.

indicators:ISO37122ClauseSixteenPointFive
	a
		owl:Class ,
		sh:NodeShape
		;
	rdfs:subClassOf indicators:SolidWasteIndicator ;
	rdfs:label "ISO37122ClauseSixteenPointFive"@en ;
	rdfs:comment "ISO 37122:2019 Clause 16.5 - Percentage of public garbage bins that are sensor-enabled public garbage bins."@en ;
	sh:targetClass indicators:ISO37122ClauseSixteenPointFive ;
	.

indicators:ISO37122ClauseSixteenPointFour
	a
		owl:Class ,
		sh:NodeShape
		;
	rdfs:subClassOf indicators:SolidWasteIndicator ;
	rdfs:label "ISO37122ClauseSixteenPointFour"@en ;
	rdfs:comment "ISO 37122:2019 Clause 16.4 - Percentage of total amount of plastic waste recycled in the city."@en ;
	sh:targetClass indicators:ISO37122ClauseSixteenPointFour ;
	.

indicators:ISO37122ClauseSixteenPointOne
	a
		owl:Class ,
		sh:NodeShape
		;
	rdfs:subClassOf indicators:SolidWasteIndicator ;
	rdfs:label "ISO37122ClauseSixteenPointOne"@en ;
	rdfs:comment "ISO 37122:2019 Clause 16.1 - Percentage of waste drop-off centres (containers) equipped with telemetering."@en-gb ;
	sh:targetClass indicators:ISO37122ClauseSixteenPointOne ;
	.

indicators:ISO37122ClauseSixteenPointSix
	a
		owl:Class ,
		sh:NodeShape
		;
	rdfs:subClassOf indicators:SolidWasteIndicator ;
	rdfs:label "ISO37122ClauseSixteenPointSix"@en ;
	rdfs:comment "ISO 37122:2019 Clause 16.6 - Percentage of the city’s electrical and electronic waste that is recycled."@en ;
	sh:targetClass indicators:ISO37122ClauseSixteenPointSix ;
	.

indicators:ISO37122ClauseSixteenPointThree
	a
		owl:Class ,
		sh:NodeShape
		;
	rdfs:subClassOf indicators:SolidWasteIndicator ;
	rdfs:label "ISO37122ClauseSixteenPointThree"@en ;
	rdfs:comment "ISO 37122:2019 Clause 16.3 - Percentage of total amount of waste in the city that is used to generate energy."@en ;
	sh:targetClass indicators:ISO37122ClauseSixteenPointThree ;
	.

indicators:ISO37122ClauseSixteenPointTwo
	a
		owl:Class ,
		sh:NodeShape
		;
	rdfs:subClassOf indicators:SolidWasteIndicator ;
	rdfs:label "ISO37122ClauseSixteenPointTwo"@en ;
	rdfs:comment "ISO 37122:2019 Clause 16.2 - Percentage of the city population that has a door-to-door garbage collection with an individual monitoring of household waste quantities."@en ;
	sh:targetClass indicators:ISO37122ClauseSixteenPointTwo ;
	.

indicators:ISO37122ClauseTenPointFour
	a
		owl:Class ,
		sh:NodeShape
		;
	rdfs:subClassOf indicators:GovernanceIndicator ;
	rdfs:label "ISO37122ClauseTenPointFour"@en ;
	rdfs:comment "ISO 37122:2019 Clause 10.4 - Average downtime of the city’s IT infrastructure."@en ;
	sh:targetClass indicators:ISO37122ClauseTenPointFour ;
	.

indicators:ISO37122ClauseTenPointOne
	a
		owl:Class ,
		sh:NodeShape
		;
	rdfs:subClassOf indicators:GovernanceIndicator ;
	rdfs:label "ISO37122ClauseTenPointOne"@en ;
	rdfs:comment "ISO 37122:2019 Clause 10.1 - Annual number of online visits to the municipal open data portal per 100 000 population."@en ;
	sh:targetClass indicators:ISO37122ClauseTenPointOne ;
	.

indicators:ISO37122ClauseTenPointThree
	a
		owl:Class ,
		sh:NodeShape
		;
	rdfs:subClassOf indicators:GovernanceIndicator ;
	rdfs:label "ISO37122ClauseTenPointThree"@en ;
	rdfs:comment "ISO 37122:2019 Clause 10.3 - Average response time to inquiries made through the city’s non-emergency inquiry system (days)."@en ;
	sh:targetClass indicators:ISO37122ClauseTenPointThree ;
	.

indicators:ISO37122ClauseTenPointTwo
	a
		owl:Class ,
		sh:NodeShape
		;
	rdfs:subClassOf indicators:GovernanceIndicator ;
	rdfs:label "ISO37122ClauseTenPointTwo"@en ;
	rdfs:comment "ISO 37122:2019 Clause 10.2 -Percentage of city services accessible and that can be requested online."@en ;
	sh:targetClass indicators:ISO37122ClauseTenPointTwo ;
	.

indicators:ISO37122ClauseThirteenPointFour
	a
		owl:Class ,
		sh:NodeShape
		;
	rdfs:subClassOf indicators:PopulationAndSocialConditionIndicator ;
	rdfs:label "ISO37122ClauseThirteenPointFour"@en ;
	rdfs:comment "ISO 37122:2019 Clause 13.4 - Percentage of municipal budget allocated for provision of programmes designated for bridging the digital divide."@en-gb ;
	sh:targetClass indicators:ISO37122ClauseThirteenPointFour ;
	.

indicators:ISO37122ClauseThirteenPointOne
	a
		owl:Class ,
		sh:NodeShape
		;
	rdfs:subClassOf indicators:PopulationAndSocialConditionIndicator ;
	rdfs:label "ISO37122ClauseThirteenPointOne"@en ;
	rdfs:comment "ISO 37122:2019 Clause 13.1 - Percentage of public buildings that are accessible by persons with special needs."@en ;
	sh:targetClass indicators:ISO37122ClauseThirteenPointOne ;
	.

indicators:ISO37122ClauseThirteenPointThree
	a
		owl:Class ,
		sh:NodeShape
		;
	rdfs:subClassOf indicators:PopulationAndSocialConditionIndicator ;
	rdfs:label "ISO37122ClauseThirteenPointThree"@en ;
	rdfs:comment "ISO 37122:2019 Clause 13.3 - Percentage of marked pedestrian crossings equipped with accessible pedestrian signals."@en ;
	sh:targetClass indicators:ISO37122ClauseThirteenPointThree ;
	.

indicators:ISO37122ClauseThirteenPointTwo
	a
		owl:Class ,
		sh:NodeShape
		;
	rdfs:subClassOf indicators:PopulationAndSocialConditionIndicator ;
	rdfs:label "ISO37122ClauseThirteenPointTwo"@en ;
	rdfs:comment "ISO 37122:2019 Clause 13.2 - Percentage of municipal budget allocated for the provision of mobility aids, devices and assistive technologies to citizens with special needs."@en ;
	sh:targetClass indicators:ISO37122ClauseThirteenPointTwo ;
	.

indicators:ISO37122ClauseTwelvePointOne
	a
		owl:Class ,
		sh:NodeShape
		;
	rdfs:subClassOf indicators:HousingIndicator ;
	rdfs:label "ISO37122ClauseTwelvePointOne"@en ;
	rdfs:comment "ISO 37122:2019 Clause 12.1 - Percentage of households with smart energy meters."@en ;
	sh:targetClass indicators:ISO37122ClauseTwelvePointOne ;
	.

indicators:ISO37122ClauseTwelvePointTwo
	a
		owl:Class ,
		sh:NodeShape
		;
	rdfs:subClassOf indicators:HousingIndicator ;
	rdfs:label "ISO37122ClauseTwelvePointTwo"@en ;
	rdfs:comment "ISO 37122:2019 Clause 12.2 - Percentage of households with smart water meters."@en ;
	sh:targetClass indicators:ISO37122ClauseTwelvePointTwo ;
	.

indicators:ISO37122ClauseTwentyOnePointFour
	a
		owl:Class ,
		sh:NodeShape
		;
	rdfs:subClassOf indicators:UrbanPlanningIndicator ;
	rdfs:label "ISO37122ClauseTwentyOnePointFour"@en ;
	rdfs:comment "ISO 37122:2019 Clause 21.4 - Percentage of the city population living in medium-to-high population densities."@en ;
	sh:targetClass indicators:ISO37122ClauseTwentyOnePointFour ;
	.

indicators:ISO37122ClauseTwentyOnePointOne
	a
		owl:Class ,
		sh:NodeShape
		;
	rdfs:subClassOf indicators:UrbanPlanningIndicator ;
	rdfs:label "ISO37122ClauseTwentyOnePointOne"@en ;
	rdfs:comment "ISO 37122:2019 Clause 21.1 - Annual number of citizens engaged in the planning process per 100 000 population."@en ;
	sh:targetClass indicators:ISO37122ClauseTwentyOnePointOne ;
	.

indicators:ISO37122ClauseTwentyOnePointThree
	a
		owl:Class ,
		sh:NodeShape
		;
	rdfs:subClassOf indicators:UrbanPlanningIndicator ;
	rdfs:label "ISO37122ClauseTwentyOnePointThree"@en ;
	rdfs:comment "ISO 37122:2019 Clause 21.3 - Average time for building permit approval (days)."@en ;
	sh:targetClass indicators:ISO37122ClauseTwentyOnePointThree ;
	.

indicators:ISO37122ClauseTwentyOnePointTwo
	a
		owl:Class ,
		sh:NodeShape
		;
	rdfs:subClassOf indicators:UrbanPlanningIndicator ;
	rdfs:label "ISO37122ClauseTwentyOnePointTwo"@en ;
	rdfs:comment "ISO 37122:2019 Clause 21.2 - Percentage of building permits submitted through an electronic submission system."@en ;
	sh:targetClass indicators:ISO37122ClauseTwentyOnePointTwo ;
	.

indicators:ISO37122ClauseTwentyPointOne
	a
		owl:Class ,
		sh:NodeShape
		;
	rdfs:subClassOf indicators:UrbanLocalAgricultureAndFoodSecurityIndicator ;
	rdfs:label "ISO37122ClauseTwentyPointOne"@en ;
	rdfs:comment "ISO 37122:2019 Clause 20.1 - Annual percentage of municipal budget spent on urban agriculture initiatives."@en ;
	sh:targetClass indicators:ISO37122ClauseTwentyPointOne ;
	.

indicators:ISO37122ClauseTwentyPointThree
	a
		owl:Class ,
		sh:NodeShape
		;
	rdfs:subClassOf indicators:UrbanLocalAgricultureAndFoodSecurityIndicator ;
	rdfs:label "ISO37122ClauseTwentyPointThree"@en ;
	rdfs:comment "ISO 37122:2019 Clause 20.3 - Percentage of the city’s land area covered by an online food-supplier mapping system."@en ;
	sh:targetClass indicators:ISO37122ClauseTwentyPointThree ;
	.

indicators:ISO37122ClauseTwentyPointTwo
	a
		owl:Class ,
		sh:NodeShape
		;
	rdfs:subClassOf indicators:UrbanLocalAgricultureAndFoodSecurityIndicator ;
	rdfs:label "ISO37122ClauseTwentyPointTwo"@en ;
	rdfs:comment "ISO 37122:2019 Clause 20.2 - Annual total collected municipal food waste sent to a processing facility for composting per capita (in tonnes)."@en-gb ;
	sh:targetClass indicators:ISO37122ClauseTwentyPointTwo ;
	.

indicators:ISO37122ClauseTwentyThreePointFour
	a
		owl:Class ,
		sh:NodeShape
		;
	rdfs:subClassOf indicators:WaterIndicator ;
	rdfs:label "ISO37122ClauseTwentyThreePointFour"@en ;
	rdfs:comment "ISO 37122:2019 Clause 23.4 - Percentage of buildings in the city with smart water meters."@en ;
	sh:targetClass indicators:ISO37122ClauseTwentyThreePointFour ;
	.

indicators:ISO37122ClauseTwentyThreePointOne
	a
		owl:Class ,
		sh:NodeShape
		;
	rdfs:subClassOf indicators:WaterIndicator ;
	rdfs:label "ISO37122ClauseTwentyThreePointOne"@en ;
	rdfs:comment "ISO 37122:2019 Clause 23.1 - Percentage of drinking water tracked by real-time, water quality monitoring station."@en ;
	sh:targetClass indicators:ISO37122ClauseTwentyThreePointOne ;
	.

indicators:ISO37122ClauseTwentyThreePointThree
	a
		owl:Class ,
		sh:NodeShape
		;
	rdfs:subClassOf indicators:WaterIndicator ;
	rdfs:label "ISO37122ClauseTwentyThreePointThree"@en ;
	rdfs:comment "ISO 37122:2019 Clause 23.3 - Percentage of the city’s water distribution network monitored by a smart water system."@en ;
	sh:targetClass indicators:ISO37122ClauseTwentyThreePointThree ;
	.

indicators:ISO37122ClauseTwentyThreePointTwo
	a
		owl:Class ,
		sh:NodeShape
		;
	rdfs:subClassOf indicators:WaterIndicator ;
	rdfs:label "ISO37122ClauseTwentyThreePointTwo"@en ;
	rdfs:comment "ISO 37122:2019 Clause 23.2 - Number of real-time environmental water quality monitoring stations per 100 000 population."@en ;
	sh:targetClass indicators:ISO37122ClauseTwentyThreePointTwo ;
	.

indicators:ISO37122ClauseTwentyTwoPointFive
	a
		owl:Class ,
		sh:NodeShape
		;
	rdfs:subClassOf indicators:WastewaterIndicator ;
	rdfs:label "ISO37122ClauseTwentyTwoPointFive"@en ;
	rdfs:comment "ISO 37122:2019 Clause 22.5 - Percentage of the wastewater pipeline network monitored by a real-time data-tracking sensor system."@en ;
	sh:targetClass indicators:ISO37122ClauseTwentyTwoPointFive ;
	.

indicators:ISO37122ClauseTwentyTwoPointFour
	a
		owl:Class ,
		sh:NodeShape
		;
	rdfs:subClassOf indicators:WastewaterIndicator ;
	rdfs:label "ISO37122ClauseTwentyTwoPointFour"@en ;
	rdfs:comment "ISO 37122:2019 Clause 22.4 - Percentage of total amount of wastewater in the city that is used to generate energy."@en ;
	sh:targetClass indicators:ISO37122ClauseTwentyTwoPointFour ;
	.

indicators:ISO37122ClauseTwentyTwoPointOne
	a
		owl:Class ,
		sh:NodeShape
		;
	rdfs:subClassOf indicators:WastewaterIndicator ;
	rdfs:label "ISO37122ClauseTwentyTwoPointOne"@en ;
	rdfs:comment "ISO 37122:2019 Clause 22.1 - Percentage of treated wastewater being reused."@en ;
	sh:targetClass indicators:ISO37122ClauseTwentyTwoPointOne ;
	.

indicators:ISO37122ClauseTwentyTwoPointThree
	a
		owl:Class ,
		sh:NodeShape
		;
	rdfs:subClassOf indicators:WastewaterIndicator ;
	rdfs:label "ISO37122ClauseTwentyTwoPointThree"@en ;
	rdfs:comment "ISO 37122:2019 Clause 22.3 - Energy derived from wastewater as a percentage of total energy consumption of the city."@en ;
	sh:targetClass indicators:ISO37122ClauseTwentyTwoPointThree ;
	.

indicators:ISO37122ClauseTwentyTwoPointTwo
	a
		owl:Class ,
		sh:NodeShape
		;
	rdfs:subClassOf indicators:WastewaterIndicator ;
	rdfs:label "ISO37122ClauseTwentyTwoPointTwo"@en ;
	rdfs:comment "ISO 37122:2019 Clause 22.2 - Percentage of biosolids that are reused (dry matter mass)."@en ;
	sh:targetClass indicators:ISO37122ClauseTwentyTwoPointTwo ;
	.

indicators:ISO37123ClauseEightPointEight
	a
		owl:Class ,
		sh:NodeShape
		;
	rdfs:subClassOf indicators:EnvironmentAndClimateChangeIndicator ;
	rdfs:label "ISO37123ClauseEightPointEight"@en ;
	rdfs:comment "ISO 37123:2019 Clause 8.8 - Percentage of city land area covered by tree canopy."@en ;
	sh:targetClass indicators:ISO37123ClauseEightPointEight ;
	.

indicators:ISO37123ClauseEightPointFive
	a
		owl:Class ,
		sh:NodeShape
		;
	rdfs:subClassOf indicators:EnvironmentAndClimateChangeIndicator ;
	rdfs:label "ISO37123ClauseEightPointFive"@en ;
	rdfs:comment "ISO 37123:2019 Clause 8.5 - Annual frequency of extreme heat events."@en ;
	sh:targetClass indicators:ISO37123ClauseEightPointFive ;
	.

indicators:ISO37123ClauseEightPointFour
	a
		owl:Class ,
		sh:NodeShape
		;
	rdfs:subClassOf indicators:EnvironmentAndClimateChangeIndicator ;
	rdfs:label "ISO37123ClauseEightPointFour"@en ;
	rdfs:comment "ISO 37123:2019 Clause 8.4 - Annual frequency of extreme rainfall events."@en ;
	sh:targetClass indicators:ISO37123ClauseEightPointFour ;
	.

indicators:ISO37123ClauseEightPointNine
	a
		owl:Class ,
		sh:NodeShape
		;
	rdfs:subClassOf indicators:EnvironmentAndClimateChangeIndicator ;
	rdfs:label "ISO37123ClauseEightPointNine"@en ;
	rdfs:comment "ISO 37123:2019 Clause 8.9 - Percentage of city surface area covered with high-albedo materials contributing to the mitigation of urban heat islands."@en ;
	sh:targetClass indicators:ISO37123ClauseEightPointNine ;
	.

indicators:ISO37123ClauseEightPointOne
	a
		owl:Class ,
		sh:NodeShape
		;
	rdfs:subClassOf indicators:EnvironmentAndClimateChangeIndicator ;
	rdfs:label "ISO37123ClauseEightPointOne"@en ;
	rdfs:comment "ISO 37123:2019 Clause 8.1 - Magnitude of urban heat island effects (atmospheric)."@en ;
	sh:targetClass indicators:ISO37123ClauseEightPointOne ;
	.

indicators:ISO37123ClauseEightPointSeven
	a
		owl:Class ,
		sh:NodeShape
		;
	rdfs:subClassOf indicators:EnvironmentAndClimateChangeIndicator ;
	rdfs:label "ISO37123ClauseEightPointSeven"@en ;
	rdfs:comment "ISO 37123:2019 Clause 8.7 - Annual frequency of flood events."@en ;
	sh:targetClass indicators:ISO37123ClauseEightPointSeven ;
	.

indicators:ISO37123ClauseEightPointSix
	a
		owl:Class ,
		sh:NodeShape
		;
	rdfs:subClassOf indicators:EnvironmentAndClimateChangeIndicator ;
	rdfs:label "ISO37123ClauseEightPointSix"@en ;
	rdfs:comment "ISO 37123:2019 Clause 8.6 - Annual frequency of extreme cold events."@en ;
	sh:targetClass indicators:ISO37123ClauseEightPointSix ;
	.

indicators:ISO37123ClauseEightPointThree
	a
		owl:Class ,
		sh:NodeShape
		;
	rdfs:subClassOf indicators:EnvironmentAndClimateChangeIndicator ;
	rdfs:label "ISO37123ClauseEightPointThree"@en ;
	rdfs:comment "ISO 37123:2019 Clause 8.3 - Territory undergoing ecosystem restoration as a percentage of total city area."@en ;
	sh:targetClass indicators:ISO37123ClauseEightPointThree ;
	.

indicators:ISO37123ClauseEightPointTwo
	a
		owl:Class ,
		sh:NodeShape
		;
	rdfs:subClassOf indicators:EnvironmentAndClimateChangeIndicator ;
	rdfs:label "ISO37123ClauseEightPointTwo"@en ;
	rdfs:comment "ISO 37123:2019 Clause 8.2 - Percentage of natural areas within the city that have undergone ecological evaluation for their protective services."@en ;
	sh:targetClass indicators:ISO37123ClauseEightPointTwo ;
	.

indicators:ISO37123ClauseEighteenPointOne
	a
		owl:Class ,
		sh:NodeShape
		;
	rdfs:subClassOf indicators:TelecommunicationIndicator ;
	rdfs:label "ISO37123ClauseEighteenPointOne"@en ;
	rdfs:comment "ISO 37123:2019 Clause 18.1 - Percentage of emergency responders in the city equipped with specialized communication technologies able to operate reliably during a disaster event."@en-us ;
	sh:targetClass indicators:ISO37123ClauseEighteenPointOne ;
	.

indicators:ISO37123ClauseElevenPointFour
	a
		owl:Class ,
		sh:NodeShape
		;
	rdfs:subClassOf indicators:HealthIndicator ;
	rdfs:label "ISO37123ClauseElevenPointFour"@en ;
	rdfs:comment "ISO 37123:2019 Clause 11.4 - Number of infectious disease outbreaks per year."@en ;
	sh:targetClass indicators:ISO37123ClauseElevenPointFour ;
	.

indicators:ISO37123ClauseElevenPointOne
	a
		owl:Class ,
		sh:NodeShape
		;
	rdfs:subClassOf indicators:HealthIndicator ;
	rdfs:label "ISO37123ClauseElevenPointOne"@en ;
	rdfs:comment "ISO 37123:2019 Clause 11.1 - Percentage of hospitals equipped with back-up electricity supply."@en ;
	sh:targetClass indicators:ISO37123ClauseElevenPointOne ;
	.

indicators:ISO37123ClauseElevenPointThree
	a
		owl:Class ,
		sh:NodeShape
		;
	rdfs:subClassOf indicators:HealthIndicator ;
	rdfs:label "ISO37123ClauseElevenPointThree"@en ;
	rdfs:comment "ISO 37123:2019 Clause 11.3 - Percentage of population that is fully immunized."@en-us ;
	sh:targetClass indicators:ISO37123ClauseElevenPointThree ;
	.

indicators:ISO37123ClauseElevenPointTwo
	a
		owl:Class ,
		sh:NodeShape
		;
	rdfs:subClassOf indicators:HealthIndicator ;
	rdfs:label "ISO37123ClauseElevenPointTwo"@en ;
	rdfs:comment "ISO 37123:2019 Clause 11.2 - Percentage of population with basic health insurance."@en ;
	sh:targetClass indicators:ISO37123ClauseElevenPointTwo ;
	.

indicators:ISO37123ClauseFifteenPointFour
	a
		owl:Class ,
		sh:NodeShape
		;
	rdfs:subClassOf indicators:SafetyIndicator ;
	rdfs:label "ISO37123ClauseFifteenPointFour"@en ;
	rdfs:comment "ISO 37123:2019 Clause 15.4 - Number of hospital beds in the city destroyed or damaged by natural hazards per 100 000 population."@en ;
	sh:targetClass indicators:ISO37123ClauseFifteenPointFour ;
	.

indicators:ISO37123ClauseFifteenPointOne
	a
		owl:Class ,
		sh:NodeShape
		;
	rdfs:subClassOf indicators:SafetyIndicator ;
	rdfs:label "ISO37123ClauseFifteenPointOne"@en ;
	rdfs:comment "ISO 37123:2019 Clause 15.1 - Percentage of city population covered by multi-hazard early warning system."@en ;
	sh:targetClass indicators:ISO37123ClauseFifteenPointOne ;
	.

indicators:ISO37123ClauseFifteenPointThree
	a
		owl:Class ,
		sh:NodeShape
		;
	rdfs:subClassOf indicators:SafetyIndicator ;
	rdfs:label "ISO37123ClauseFifteenPointThree"@en ;
	rdfs:comment "ISO 37123:2019 Clause 15.3 - Percentage of local hazard warnings issued by national agencies annually that are received in a timely fashion by the city."@en ;
	sh:targetClass indicators:ISO37123ClauseFifteenPointThree ;
	.

indicators:ISO37123ClauseFifteenPointTwo
	a
		owl:Class ,
		sh:NodeShape
		;
	rdfs:subClassOf indicators:SafetyIndicator ;
	rdfs:label "ISO37123ClauseFifteenPointTwo"@en ;
	rdfs:comment "ISO 37123:2019 Clause 15.2 - Percentage of emergency responders who have received disaster response training."@en ;
	sh:targetClass indicators:ISO37123ClauseFifteenPointTwo ;
	.

indicators:ISO37123ClauseFivePointFive
	a
		owl:Class ,
		sh:NodeShape
		;
	rdfs:subClassOf indicators:EconomyIndicator ;
	rdfs:label "ISO37123ClauseFivePointFive"@en ;
	rdfs:comment "ISO 37123:2019 Clause 5.5 - Employment concentration."@en ;
	sh:targetClass indicators:ISO37123ClauseFivePointFive ;
	.

indicators:ISO37123ClauseFivePointFour
	a
		owl:Class ,
		sh:NodeShape
		;
	rdfs:subClassOf indicators:EconomyIndicator ;
	rdfs:label "ISO37123ClauseFivePointFour"@en ;
	rdfs:comment "ISO 37123:2019 Clause 5.4 - Percentage of total insured value to total value at risk within the city."@en ;
	sh:targetClass indicators:ISO37123ClauseFivePointFour ;
	.

indicators:ISO37123ClauseFivePointOne
	a
		owl:Class ,
		sh:NodeShape
		;
	rdfs:subClassOf indicators:EconomyIndicator ;
	rdfs:label "ISO37123ClauseFivePointOne"@en ;
	rdfs:comment "ISO 37123:2019 Clause 5.1 - Historical disaster losses as a percentage of city product."@en ;
	sh:targetClass indicators:ISO37123ClauseFivePointOne ;
	.

indicators:ISO37123ClauseFivePointSeven
	a
		owl:Class ,
		sh:NodeShape
		;
	rdfs:subClassOf indicators:EconomyIndicator ;
	rdfs:label "ISO37123ClauseFivePointSeven"@en ;
	rdfs:comment "ISO 37123:2019 Clause 5.7 - Average household disposable income."@en ;
	sh:targetClass indicators:ISO37123ClauseFivePointSeven ;
	.

indicators:ISO37123ClauseFivePointSix
	a
		owl:Class ,
		sh:NodeShape
		;
	rdfs:subClassOf indicators:EconomyIndicator ;
	rdfs:label "ISO37123ClauseFivePointSix"@en ;
	rdfs:comment "ISO 37123:2019 Clause 5.6 - Percentage of the workforce in informal employment."@en ;
	sh:targetClass indicators:ISO37123ClauseFivePointSix ;
	.

indicators:ISO37123ClauseFivePointThree
	a
		owl:Class ,
		sh:NodeShape
		;
	rdfs:subClassOf indicators:EconomyIndicator ;
	rdfs:label "ISO37123ClauseFivePointThree"@en ;
	rdfs:comment "ISO 37123:2019 Clause 5.3 - Percentage of properties with insurance coverage for high-risk hazard."@en ;
	sh:targetClass indicators:ISO37123ClauseFivePointThree ;
	.

indicators:ISO37123ClauseFivePointTwo
	a
		owl:Class ,
		sh:NodeShape
		;
	rdfs:subClassOf indicators:EconomyIndicator ;
	rdfs:label "ISO37123ClauseFivePointTwo"@en ;
	rdfs:comment "ISO 37123:2019 Clause 5.2 - Average annual disaster loss as a percentage of city product."@en ;
	sh:targetClass indicators:ISO37123ClauseFivePointTwo ;
	.

indicators:ISO37123ClauseFourteenPointOne
	a
		owl:Class ,
		sh:NodeShape
		;
	rdfs:subClassOf indicators:RecreationIndicator ;
	rdfs:label "ISO37123ClauseFourteenPointOne"@en ;
	rdfs:comment "ISO 37123:2019 Clause 14.1 - Square metres of public indoor recreation space per capita (supporting indicator). [Note: This indicator is indentical to ISO 37120, Clause 14.1 as specified by ISO 37123:2019]."@en-gb ;
	sh:targetClass indicators:ISO37123ClauseFourteenPointOne ;
	.

indicators:ISO37123ClauseFourteenPointTwo
	a
		owl:Class ,
		sh:NodeShape
		;
	rdfs:subClassOf indicators:RecreationIndicator ;
	rdfs:label "ISO37123ClauseFourteenPointTwo"@en ;
	rdfs:comment "ISO 37123:2019 Clause 14.2 - Square metres of public outdoor recreation space per capita (supporting indicator). [Note: This indicator is indentical to ISO 37120, Clause 14.1 as specified by ISO 37123:2019]."@en-gb ;
	sh:targetClass indicators:ISO37123ClauseFourteenPointTwo ;
	.

indicators:ISO37123ClauseNinePointFive
	a
		owl:Class ,
		sh:NodeShape
		;
	rdfs:subClassOf indicators:FinanceIndicator ;
	rdfs:label "ISO37123ClauseNinePointFive"@en ;
	rdfs:comment "ISO 37123:2019 Clause 9.5 - Annual expenditure on emergency management planning as a percentage of total city budget."@en ;
	sh:targetClass indicators:ISO37123ClauseNinePointFive ;
	.

indicators:ISO37123ClauseNinePointFour
	a
		owl:Class ,
		sh:NodeShape
		;
	rdfs:subClassOf indicators:FinanceIndicator ;
	rdfs:label "ISO37123ClauseNinePointFour"@en ;
	rdfs:comment "ISO 37123:2019 Clause 9.4 - Annual expenditure on green and blue infrastructure as a percentage of total city budget."@en ;
	sh:targetClass indicators:ISO37123ClauseNinePointFour ;
	.

indicators:ISO37123ClauseNinePointOne
	a
		owl:Class ,
		sh:NodeShape
		;
	rdfs:subClassOf indicators:FinanceIndicator ;
	rdfs:label "ISO37123ClauseNinePointOne"@en ;
	rdfs:comment "ISO 37123:2019 Clause 9.1 - Annual expenditure on upgrades and maintenance of city service assets as a percentage of total city budget."@en ;
	sh:targetClass indicators:ISO37123ClauseNinePointOne ;
	.

indicators:ISO37123ClauseNinePointSeven
	a
		owl:Class ,
		sh:NodeShape
		;
	rdfs:subClassOf indicators:FinanceIndicator ;
	rdfs:label "ISO37123ClauseNinePointSeven"@en ;
	rdfs:comment "ISO 37123:2019 Clause 9.7 - Total allocation of disaster reserve funds as a percentage of total city budget."@en ;
	sh:targetClass indicators:ISO37123ClauseNinePointSeven ;
	.

indicators:ISO37123ClauseNinePointSix
	a
		owl:Class ,
		sh:NodeShape
		;
	rdfs:subClassOf indicators:FinanceIndicator ;
	rdfs:label "ISO37123ClauseNinePointSix"@en ;
	rdfs:comment "ISO 37123:2019 Clause 9.6 - Noise pollution (supporting indicator)."@en ;
	sh:targetClass indicators:ISO37123ClauseNinePointSix ;
	.

indicators:ISO37123ClauseNinePointThree
	a
		owl:Class ,
		sh:NodeShape
		;
	rdfs:subClassOf indicators:FinanceIndicator ;
	rdfs:label "ISO37123ClauseNinePointThree"@en ;
	rdfs:comment "ISO 37123:2019 Clause 9.3 - Annual expenditure allocated to ecosystem restoration in the city’s territory as a percentage of total city budget."@en ;
	sh:targetClass indicators:ISO37123ClauseNinePointThree ;
	.

indicators:ISO37123ClauseNinePointTwo
	a
		owl:Class ,
		sh:NodeShape
		;
	rdfs:subClassOf indicators:FinanceIndicator ;
	rdfs:label "ISO37123ClauseNinePointTwo"@en ;
	rdfs:comment "ISO 37123:2019 Clause 9.2 - Annual expenditure on upgrades and maintenance of storm water infrastructure as a percentage of total city budget."@en ;
	sh:targetClass indicators:ISO37123ClauseNinePointTwo ;
	.

indicators:ISO37123ClauseNineteenPointOne
	a
		owl:Class ,
		sh:NodeShape
		;
	rdfs:subClassOf indicators:TransportationIndicator ;
	rdfs:label "ISO37123ClauseNineteenPointOne"@en ;
	rdfs:comment "ISO 37123:2019 Clause 19.1 - Number of evacuation routes available per 100 000 population."@en ;
	sh:targetClass indicators:ISO37123ClauseNineteenPointOne ;
	.

indicators:ISO37123ClauseSevenPointOne
	a
		owl:Class ,
		sh:NodeShape
		;
	rdfs:subClassOf indicators:EnergyIndicator ;
	rdfs:label "ISO37123ClauseSevenPointOne"@en ;
	rdfs:comment "ISO 37123:2019 Clause 7.1 - Number of different electricity sources providing at least 5 % of total energy supply capacity."@en ;
	sh:targetClass indicators:ISO37123ClauseSevenPointOne ;
	.

indicators:ISO37123ClauseSevenPointThree
	a
		owl:Class ,
		sh:NodeShape
		;
	rdfs:subClassOf indicators:EnergyIndicator ;
	rdfs:label "ISO37123ClauseSevenPointThree"@en ;
	rdfs:comment "ISO 37123:2019 Clause 7.3 - Percentage of critical facilities served by off-grid energy services."@en ;
	sh:targetClass indicators:ISO37123ClauseSevenPointThree ;
	.

indicators:ISO37123ClauseSevenPointTwo
	a
		owl:Class ,
		sh:NodeShape
		;
	rdfs:subClassOf indicators:EnergyIndicator ;
	rdfs:label "ISO37123ClauseSevenPointTwo"@en ;
	rdfs:comment "ISO 37123:2019 Clause 7.2 - Electricity supply capacity as a percentage of peak electricity demand."@en ;
	sh:targetClass indicators:ISO37123ClauseSevenPointTwo ;
	.

indicators:ISO37123ClauseSeventeenPointOne
	a
		owl:Class ,
		sh:NodeShape
		;
	rdfs:subClassOf indicators:SportAndCultureIndicator ;
	rdfs:label "ISO37123ClauseSeventeenPointOne"@en ;
	rdfs:comment "ISO 37123:2019 Clause 17.1 - Number of cultural institutions and sporting facilities per 100 000 population (core indicator). [Note: This indicator is indentical to ISO 37120, Clause 17.1 as specified by ISO 37123:2019]."@en ;
	sh:targetClass indicators:ISO37123ClauseSeventeenPointOne ;
	.

indicators:ISO37123ClauseSeventeenPointThree
	a
		owl:Class ,
		sh:NodeShape
		;
	rdfs:subClassOf indicators:SportAndCultureIndicator ;
	rdfs:label "ISO37123ClauseSeventeenPointThree"@en ;
	rdfs:comment "ISO 37123:2019 Clause 17.3 - Annual number of cultural events per 100 000 population (e.g. exhibitions, festivals, concerts) (supporting indicator). [Note: This indicator is indentical to ISO 37120, Clause 17.3 as specified by ISO 37123:2019]."@en ;
	sh:targetClass indicators:ISO37123ClauseSeventeenPointThree ;
	.

indicators:ISO37123ClauseSeventeenPointTwo
	a
		owl:Class ,
		sh:NodeShape
		;
	rdfs:subClassOf indicators:SportAndCultureIndicator ;
	rdfs:label "ISO37123ClauseSeventeenPointTwo"@en ;
	rdfs:comment "ISO 37123:2019 Clause 17.2 - Noise pollution (supporting indicator). [Note: This indicator is indentical to ISO 37120, Clause 17.2 as specified by ISO 37123:2019]. "@en ;
	sh:targetClass indicators:ISO37123ClauseSeventeenPointTwo ;
	.

indicators:ISO37123ClauseSixPointFour
	a
		owl:Class ,
		sh:NodeShape
		;
	rdfs:subClassOf indicators:EducationIndicator ;
	rdfs:label "ISO37123ClauseSixPointFour"@en ;
	rdfs:comment "ISO 37123:2019 Clause 6.4 - Educational disruption."@en ;
	sh:targetClass indicators:ISO37123ClauseSixPointFour ;
	.

indicators:ISO37123ClauseSixPointOne
	a
		owl:Class ,
		sh:NodeShape
		;
	rdfs:subClassOf indicators:EducationIndicator ;
	rdfs:label "ISO37123ClauseSixPointOne"@en ;
	rdfs:comment "ISO 37123:2019 Clause 6.1 - Percentage of schools that teach emergency preparedness and disaster risk reduction."@en ;
	sh:targetClass indicators:ISO37123ClauseSixPointOne ;
	.

indicators:ISO37123ClauseSixPointThree
	a
		owl:Class ,
		sh:NodeShape
		;
	rdfs:subClassOf indicators:EducationIndicator ;
	rdfs:label "ISO37123ClauseSixPointThree"@en ;
	rdfs:comment "ISO 37123:2019 Clause 6.3 - Percentage of emergency preparedness publications provided in alternative languages."@en ;
	sh:targetClass indicators:ISO37123ClauseSixPointThree ;
	.

indicators:ISO37123ClauseSixPointTwo
	a
		owl:Class ,
		sh:NodeShape
		;
	rdfs:subClassOf indicators:EducationIndicator ;
	rdfs:label "ISO37123ClauseSixPointTwo"@en ;
	rdfs:comment "ISO 37123:2019 Clause 6.2 - Noise pollution (supporting indicator)."@en ;
	sh:targetClass indicators:ISO37123ClauseSixPointTwo ;
	.

indicators:ISO37123ClauseSixteenPointOne
	a
		owl:Class ,
		sh:NodeShape
		;
	rdfs:subClassOf indicators:SolidWasteIndicator ;
	rdfs:label "ISO37123ClauseSixteenPointOne"@en ;
	rdfs:comment "ISO 37123:2019 Clause 16.1 - Number of active and temporary waste management sites available for debris and rubble per square kilometre."@en-gb ;
	sh:targetClass indicators:ISO37123ClauseSixteenPointOne ;
	.

indicators:ISO37123ClauseTenPointFive
	a
		owl:Class ,
		sh:NodeShape
		;
	rdfs:subClassOf indicators:GovernanceIndicator ;
	rdfs:label "ISO37123ClauseTenPointFive"@en ;
	rdfs:comment "ISO 37123:2019 Clause 10.5 - Number of intergovernmental agreements dedicated to planning for shocks as percentage of total intergovernmental agreements."@en ;
	sh:targetClass indicators:ISO37123ClauseTenPointFive ;
	.

indicators:ISO37123ClauseTenPointFour
	a
		owl:Class ,
		sh:NodeShape
		;
	rdfs:subClassOf indicators:GovernanceIndicator ;
	rdfs:label "ISO37123ClauseTenPointFour"@en ;
	rdfs:comment "ISO 37123:2019 Clause 10.4 - Percentage of public meetings dedicated to resilience in the city."@en ;
	sh:targetClass indicators:ISO37123ClauseTenPointFour ;
	.

indicators:ISO37123ClauseTenPointOne
	a
		owl:Class ,
		sh:NodeShape
		;
	rdfs:subClassOf indicators:GovernanceIndicator ;
	rdfs:label "ISO37123ClauseTenPointOne"@en ;
	rdfs:comment "ISO 37123:2019 Clause 10.1 - Frequency with which disaster-management plans are updated."@en ;
	sh:targetClass indicators:ISO37123ClauseTenPointOne ;
	.

indicators:ISO37123ClauseTenPointSix
	a
		owl:Class ,
		sh:NodeShape
		;
	rdfs:subClassOf indicators:GovernanceIndicator ;
	rdfs:label "ISO37123ClauseTenPointSix"@en ;
	rdfs:comment "ISO 37123:2019 Clause 10.6 - Percentage of essential service providers that have a documented business continuity plan."@en ;
	sh:targetClass indicators:ISO37123ClauseTenPointSix ;
	.

indicators:ISO37123ClauseTenPointThree
	a
		owl:Class ,
		sh:NodeShape
		;
	rdfs:subClassOf indicators:GovernanceIndicator ;
	rdfs:label "ISO37123ClauseTenPointThree"@en ;
	rdfs:comment "ISO 37123:2019 Clause 10.3 - Percentage of city electronic data with secure and remote back-up storage."@en ;
	sh:targetClass indicators:ISO37123ClauseTenPointThree ;
	.

indicators:ISO37123ClauseTenPointTwo
	a
		owl:Class ,
		sh:NodeShape
		;
	rdfs:subClassOf indicators:GovernanceIndicator ;
	rdfs:label "ISO37123ClauseTenPointTwo"@en ;
	rdfs:comment "ISO 37123:2019 Clause 10.2 - Percentage of essential city services covered by a documented continuity plan."@en ;
	sh:targetClass indicators:ISO37123ClauseTenPointTwo ;
	.

indicators:ISO37123ClauseThirteenPointFive
	a
		owl:Class ,
		sh:NodeShape
		;
	rdfs:subClassOf indicators:PopulationAndSocialConditionIndicator ;
	rdfs:label "ISO37123ClauseThirteenPointFive"@en ;
	rdfs:comment "ISO 37123:2019 Clause 13.5 - Annual percentage of the city population directly affected by natural hazards."@en ;
	sh:targetClass indicators:ISO37123ClauseThirteenPointFive ;
	.

indicators:ISO37123ClauseThirteenPointFour
	a
		owl:Class ,
		sh:NodeShape
		;
	rdfs:subClassOf indicators:PopulationAndSocialConditionIndicator ;
	rdfs:label "ISO37123ClauseThirteenPointFour"@en ;
	rdfs:comment "ISO 37123:2019 Clause 13.4 - Percentage of neighbourhoods with regular and open neighbourhood association meetings."@en-gb ;
	sh:targetClass indicators:ISO37123ClauseThirteenPointFour ;
	.

indicators:ISO37123ClauseThirteenPointOne
	a
		owl:Class ,
		sh:NodeShape
		;
	rdfs:subClassOf indicators:PopulationAndSocialConditionIndicator ;
	rdfs:label "ISO37123ClauseThirteenPointOne"@en ;
	rdfs:comment "ISO 37123:2019 Clause 13.1 - Vulnerable population as a percentage of city population."@en ;
	sh:targetClass indicators:ISO37123ClauseThirteenPointOne ;
	.

indicators:ISO37123ClauseThirteenPointThree
	a
		owl:Class ,
		sh:NodeShape
		;
	rdfs:subClassOf indicators:PopulationAndSocialConditionIndicator ;
	rdfs:label "ISO37123ClauseThirteenPointThree"@en ;
	rdfs:comment "ISO 37123:2019 Clause 13.3 - Percentage of population at high risk from natural hazards."@en ;
	sh:targetClass indicators:ISO37123ClauseThirteenPointThree ;
	.

indicators:ISO37123ClauseThirteenPointTwo
	a
		owl:Class ,
		sh:NodeShape
		;
	rdfs:subClassOf indicators:PopulationAndSocialConditionIndicator ;
	rdfs:label "ISO37123ClauseThirteenPointTwo"@en ;
	rdfs:comment "ISO 37123:2019 Clause 13.2 - Percentage of population enrolled in social assistance programmes."@en-gb ;
	sh:targetClass indicators:ISO37123ClauseThirteenPointTwo ;
	.

indicators:ISO37123ClauseTwelvePointFive
	a
		owl:Class ,
		sh:NodeShape
		;
	rdfs:subClassOf indicators:HousingIndicator ;
	rdfs:label "ISO37123ClauseTwelvePointFive"@en ;
	rdfs:comment "ISO 37123:2019 Clause 12.5 - Annual number of residential properties flooded as a percentage of total residential properties in the city."@en ;
	sh:targetClass indicators:ISO37123ClauseTwelvePointFive ;
	.

indicators:ISO37123ClauseTwelvePointFour
	a
		owl:Class ,
		sh:NodeShape
		;
	rdfs:subClassOf indicators:HousingIndicator ;
	rdfs:label "ISO37123ClauseTwelvePointFour"@en ;
	rdfs:comment "ISO 37123:2019 Clause 12.4 - Percentage of damaged infrastructure that was “built back better” after a disaster."@en ;
	sh:targetClass indicators:ISO37123ClauseTwelvePointFour ;
	.

indicators:ISO37123ClauseTwelvePointOne
	a
		owl:Class ,
		sh:NodeShape
		;
	rdfs:subClassOf indicators:HousingIndicator ;
	rdfs:label "ISO37123ClauseTwelvePointOne"@en ;
	rdfs:comment "ISO 37123:2019 Clause 12.1 - Capacity of designated emergency shelters per 100 000 population."@en ;
	sh:targetClass indicators:ISO37123ClauseTwelvePointOne ;
	.

indicators:ISO37123ClauseTwelvePointSix
	a
		owl:Class ,
		sh:NodeShape
		;
	rdfs:subClassOf indicators:HousingIndicator ;
	rdfs:label "ISO37123ClauseTwelvePointSix"@en ;
	rdfs:comment "ISO 37123:2019 Clause 12.6 - Percentage of residential properties located in high-risk zones."@en ;
	sh:targetClass indicators:ISO37123ClauseTwelvePointSix ;
	.

indicators:ISO37123ClauseTwelvePointThree
	a
		owl:Class ,
		sh:NodeShape
		;
	rdfs:subClassOf indicators:HousingIndicator ;
	rdfs:label "ISO37123ClauseTwelvePointThree"@en ;
	rdfs:comment "ISO 37123:2019 Clause 12.3 - Percentage of residential buildings not in conformity with building codes and standards."@en ;
	sh:targetClass indicators:ISO37123ClauseTwelvePointThree ;
	.

indicators:ISO37123ClauseTwelvePointTwo
	a
		owl:Class ,
		sh:NodeShape
		;
	rdfs:subClassOf indicators:HousingIndicator ;
	rdfs:label "ISO37123ClauseTwelvePointTwo"@en ;
	rdfs:comment "ISO 37123:2019 Clause 12.2 - Percentage of buildings structurally vulnerable to high-risk hazards."@en ;
	sh:targetClass indicators:ISO37123ClauseTwelvePointTwo ;
	.

indicators:ISO37123ClauseTwentyOnePointFive
	a
		owl:Class ,
		sh:NodeShape
		;
	rdfs:subClassOf indicators:UrbanPlanningIndicator ;
	rdfs:label "ISO37123ClauseTwentyOnePointFive"@en ;
	rdfs:comment "ISO 37123:2019 Clause 21.5 - Annual number of critical infrastructures flooded as a percentage of critical infrastructure in the city."@en ;
	sh:targetClass indicators:ISO37123ClauseTwentyOnePointFive ;
	.

indicators:ISO37123ClauseTwentyOnePointFour
	a
		owl:Class ,
		sh:NodeShape
		;
	rdfs:subClassOf indicators:UrbanPlanningIndicator ;
	rdfs:label "ISO37123ClauseTwentyOnePointFour"@en ;
	rdfs:comment "ISO 37123:2019 Clause 21.4 - Percentage of city departments and utility services that conduct risk assessment in their planning and investment."@en ;
	sh:targetClass indicators:ISO37123ClauseTwentyOnePointFour ;
	.

indicators:ISO37123ClauseTwentyOnePointOne
	a
		owl:Class ,
		sh:NodeShape
		;
	rdfs:subClassOf indicators:UrbanPlanningIndicator ;
	rdfs:label "ISO37123ClauseTwentyOnePointOne"@en ;
	rdfs:comment "ISO 37123:2019 Clause 21.1 - Percentage of city area covered by publicly available hazard maps."@en ;
	sh:targetClass indicators:ISO37123ClauseTwentyOnePointOne ;
	.

indicators:ISO37123ClauseTwentyOnePointSix
	a
		owl:Class ,
		sh:NodeShape
		;
	rdfs:subClassOf indicators:UrbanPlanningIndicator ;
	rdfs:label "ISO37123ClauseTwentyOnePointSix"@en ;
	rdfs:comment "ISO 37123:2019 Clause 21.6 - Annual expenditure on water retention measures as a percentage of city prevention measures budget."@en ;
	sh:targetClass indicators:ISO37123ClauseTwentyOnePointSix ;
	.

indicators:ISO37123ClauseTwentyOnePointThree
	a
		owl:Class ,
		sh:NodeShape
		;
	rdfs:subClassOf indicators:UrbanPlanningIndicator ;
	rdfs:label "ISO37123ClauseTwentyOnePointThree"@en ;
	rdfs:comment "ISO 37123:2019 Clause 21.3 - Percentage of city land area in high-risk zones where risk-reduction measures have been implemented."@en ;
	sh:targetClass indicators:ISO37123ClauseTwentyOnePointThree ;
	.

indicators:ISO37123ClauseTwentyOnePointTwo
	a
		owl:Class ,
		sh:NodeShape
		;
	rdfs:subClassOf indicators:UrbanPlanningIndicator ;
	rdfs:label "ISO37123ClauseTwentyOnePointTwo"@en ;
	rdfs:comment "ISO 37123:2019 Clause 21.2 - Pervious land areas and public space and pavement built with porous, draining materials as a percentage of city land area."@en ;
	sh:targetClass indicators:ISO37123ClauseTwentyOnePointTwo ;
	.

indicators:ISO37123ClauseTwentyPointOne
	a
		owl:Class ,
		sh:NodeShape
		;
	rdfs:subClassOf indicators:UrbanLocalAgricultureAndFoodSecurityIndicator ;
	rdfs:label "ISO37123ClauseTwentyPointOne"@en ;
	rdfs:comment "ISO 37123:2019 Clause 20.1 - 20.1	Percentage of city population that can be served by city food reserves for 72 hours in an emergency."@en ;
	sh:targetClass indicators:ISO37123ClauseTwentyPointOne ;
	.

indicators:ISO37123ClauseTwentyPointTwo
	a
		owl:Class ,
		sh:NodeShape
		;
	rdfs:subClassOf indicators:UrbanLocalAgricultureAndFoodSecurityIndicator ;
	rdfs:label "ISO37123ClauseTwentyPointTwo"@en ;
	rdfs:comment "ISO 37123:2019 Clause 20.2 - Percentage of the city’s population living within one kilometre of a grocery store."@en-gb ;
	sh:targetClass indicators:ISO37123ClauseTwentyPointTwo ;
	.

indicators:ISO37123ClauseTwentyThreePointOne
	a
		owl:Class ,
		sh:NodeShape
		;
	rdfs:subClassOf indicators:WaterIndicator ;
	rdfs:label "ISO37123ClauseTwentyThreePointOne"@en ;
	rdfs:comment "ISO 37123:2019 Clause 23.1 - Number of different sources providing at least 5 % of total water supply capacity."@en ;
	sh:targetClass indicators:ISO37123ClauseTwentyThreePointOne ;
	.

indicators:ISO37123ClauseTwentyThreePointTwo
	a
		owl:Class ,
		sh:NodeShape
		;
	rdfs:subClassOf indicators:WaterIndicator ;
	rdfs:label "ISO37123ClauseTwentyThreePointTwo"@en ;
	rdfs:comment "ISO 37123:2019 Clause 23.2 - Percentage of city population that can be supplied with drinking water by alternative methods for 72 hours."@en ;
	sh:targetClass indicators:ISO37123ClauseTwentyThreePointTwo ;
	.

indicators:ISO37123ClauseTwentyTwoPointFour
	a
		owl:Class ,
		sh:NodeShape
		;
	rdfs:subClassOf indicators:WastewaterIndicator ;
	rdfs:label "ISO37123ClauseTwentyTwoPointFour"@en ;
	rdfs:comment "ISO 37123:2019 Clause 22.4 - Compliance rate of wastewater treatment (supporting indicator). [Note: This indicator is indentical to ISO 37120, Clause 22.4 as specified by ISO 37123:2019]."@en ;
	sh:targetClass indicators:ISO37123ClauseTwentyTwoPointFour ;
	.

indicators:ISO37123ClauseTwentyTwoPointOne
	a
		owl:Class ,
		sh:NodeShape
		;
	rdfs:subClassOf indicators:WastewaterIndicator ;
	rdfs:label "ISO37123ClauseTwentyTwoPointOne"@en ;
	rdfs:comment "ISO 37123:2019 Clause 22.1 - Percentage of city population served by wastewater collection (core indicator). [Note: This indicator is indentical to ISO 37120, Clause 22.1 as specified by ISO 37123:2019]."@en ;
	sh:targetClass indicators:ISO37123ClauseTwentyTwoPointOne ;
	.

indicators:ISO37123ClauseTwentyTwoPointThree
	a
		owl:Class ,
		sh:NodeShape
		;
	rdfs:subClassOf indicators:WastewaterIndicator ;
	rdfs:label "ISO37123ClauseTwentyTwoPointThree"@en ;
	rdfs:comment "ISO 37123:2019 Clause 22.3 - Percentage of population with access to improved sanitation (core indicator). [Note: This indicator is indentical to ISO 37120, Clause 22.3 as specified by ISO 37123:2019]."@en ;
	sh:targetClass indicators:ISO37123ClauseTwentyTwoPointThree ;
	.

indicators:ISO37123ClauseTwentyTwoPointTwo
	a
		owl:Class ,
		sh:NodeShape
		;
	rdfs:subClassOf indicators:WastewaterIndicator ;
	rdfs:label "ISO37123ClauseTwentyTwoPointTwo"@en ;
	rdfs:comment "ISO 37123:2019 Clause 22.2 - Percentage of city’s wastewater receiving centralized treatment (core indicator). [Note: This indicator is indentical to ISO 37120, Clause 22.2 as specified by ISO 37123:2019]."@en ;
	sh:targetClass indicators:ISO37123ClauseTwentyTwoPointTwo ;
	.

indicators:LivelihoodSupportSystemIndicator
	a
		owl:Class ,
		sh:NodeShape
		;
	rdfs:subClassOf indicators:Indicator ;
	rdfs:label "LivelihoodSupportSystemIndicator"@en ;
	rdfs:comment "A set of indicators that is classified under Livelihood Support System, and contains various indicators from ISO 37120:2018, ISO 37122:2019 and ISO 37123:2019. For indicators stated in ISO 37120:2018, there are 3 further types of indicators - core, supporting and profile. Further details of these types of indicators are located at clause 3.4 of ISO 37120:2018."@en ;
	sh:targetClass indicators:LivelihoodSupportSystemIndicator ;
	.

indicators:PopulationAndSocialConditionIndicator
	a
		owl:Class ,
		sh:NodeShape
		;
	rdfs:subClassOf indicators:LivelihoodSupportSystemIndicator ;
	rdfs:label "PopulationAndSocialConditionIndicator"@en ;
	rdfs:comment "A set of indicators that is classified under Livelihood Support System, and contains various indicators under clause 13 from ISO 37120:2018, ISO 37122:2019 and ISO 37123:2019. For indicators stated in ISO 37120:2018, there are 3 further types of indicators - core, supporting and profile. Further details of these types of indicators are located at clause 3.4 of ISO 37120:2018."@en ;
	sh:targetClass indicators:PopulationAndSocialConditionIndicator ;
	.

indicators:RecreationIndicator
	a
		owl:Class ,
		sh:NodeShape
		;
	rdfs:subClassOf indicators:LivelihoodSupportSystemIndicator ;
	rdfs:label "RecreationIndicator"@en ;
	rdfs:comment "A set of indicators that is classified under Livelihood Support System, and contains various indicators under clause 14 from ISO 37120:2018, ISO 37122:2019 and ISO 37123:2019. For indicators stated in ISO 37120:2018, there are 3 further types of indicators - core, supporting and profile. Further details of these types of indicators are located at clause 3.4 of ISO 37120:2018."@en ;
	sh:targetClass indicators:RecreationIndicator ;
	.

indicators:ResourceSystemIndicator
	a
		owl:Class ,
		sh:NodeShape
		;
	rdfs:subClassOf indicators:Indicator ;
	rdfs:label "ResourceSystemIndicator"@en ;
	rdfs:comment "A set of indicators that is classified under Resource System, and contains various indicators from ISO 37120:2018, ISO 37122:2019 and ISO 37123:2019. For indicators stated in ISO 37120:2018, there are 3 further types of indicators - core, supporting and profile. Further details of these types of indicators are located at clause 3.4 of ISO 37120:2018."@en ;
	sh:targetClass indicators:ResourceSystemIndicator ;
	.

indicators:SafetyIndicator
	a
		owl:Class ,
		sh:NodeShape
		;
	rdfs:subClassOf indicators:EssentialServiceSystemIndicator ;
	rdfs:label "SafetyIndicator"@en ;
	rdfs:comment "A set of indicators that is classified under Essential Service System, and contains various indicators under clause 15 from ISO 37120:2018, ISO 37122:2019 and ISO 37123:2019. For indicators stated in ISO 37120:2018, there are 3 further types of indicators - core, supporting and profile. Further details of these types of indicators are located at clause 3.4 of ISO 37120:2018."@en ;
	sh:targetClass indicators:SafetyIndicator ;
	.

indicators:SolidWasteIndicator
	a
		owl:Class ,
		sh:NodeShape
		;
	rdfs:subClassOf indicators:EssentialServiceSystemIndicator ;
	rdfs:label "SolidWasteIndicator"@en ;
	rdfs:comment "A set of indicators that is classified under Essential Service System, and contains various indicators under clause 16 from ISO 37120:2018, ISO 37122:2019 and ISO 37123:2019. For indicators stated in ISO 37120:2018, there are 3 further types of indicators - core, supporting and profile. Further details of these types of indicators are located at clause 3.4 of ISO 37120:2018."@en ;
	sh:targetClass indicators:SolidWasteIndicator ;
	.

indicators:SportAndCultureIndicator
	a
		owl:Class ,
		sh:NodeShape
		;
	rdfs:subClassOf indicators:LivelihoodSupportSystemIndicator ;
	rdfs:label "SportAndCultureIndicator"@en ;
	rdfs:comment "A set of indicators that is classified under Livelihood Support System, and contains various indicators under clause 17 from ISO 37120:2018, ISO 37122:2019 and ISO 37123:2019. For indicators stated in ISO 37120:2018, there are 3 further types of indicators - core, supporting and profile. Further details of these types of indicators are located at clause 3.4 of ISO 37120:2018."@en ;
	sh:targetClass indicators:SportAndCultureIndicator ;
	.

indicators:TelecommunicationIndicator
	a
		owl:Class ,
		sh:NodeShape
		;
	rdfs:subClassOf indicators:EssentialServiceSystemIndicator ;
	rdfs:label "TelecommunicationIndicator"@en ;
	rdfs:comment "A set of indicators that is classified under Essential Service System, and contains various indicators under clause 18 from ISO 37120:2018, ISO 37122:2019 and ISO 37123:2019. For indicators stated in ISO 37120:2018, there are 3 further types of indicators - core, supporting and profile. Further details of these types of indicators are located at clause 3.4 of ISO 37120:2018."@en ;
	sh:targetClass indicators:TelecommunicationIndicator ;
	.

indicators:TransportationIndicator
	a
		owl:Class ,
		sh:NodeShape
		;
	rdfs:subClassOf indicators:EssentialServiceSystemIndicator ;
	rdfs:label "TransportationIndicator"@en ;
	rdfs:comment "A set of indicators that is classified under Essential Service System, and contains various indicators under clause 19 from ISO 37120:2018, ISO 37122:2019 and ISO 37123:2019. For indicators stated in ISO 37120:2018, there are 3 further types of indicators - core, supporting and profile. Further details of these types of indicators are located at clause 3.4 of ISO 37120:2018."@en ;
	sh:targetClass indicators:TransportationIndicator ;
	.

indicators:UrbanLocalAgricultureAndFoodSecurityIndicator
	a
		owl:Class ,
		sh:NodeShape
		;
	rdfs:subClassOf indicators:LivelihoodSupportSystemIndicator ;
	rdfs:label "UrbanLocalAgricultureAndFoodSecurityIndicator"@en ;
	rdfs:comment "A set of indicators that is classified under Livelihood Support System, and contains various indicators under clause 20 from ISO 37120:2018, ISO 37122:2019 and ISO 37123:2019. For indicators stated in ISO 37120:2018, there are 3 further types of indicators - core, supporting and profile. Further details of these types of indicators are located at clause 3.4 of ISO 37120:2018."@en ;
	sh:targetClass indicators:UrbanLocalAgricultureAndFoodSecurityIndicator ;
	.

indicators:UrbanPlanningIndicator
	a
		owl:Class ,
		sh:NodeShape
		;
	rdfs:subClassOf indicators:LivelihoodSupportSystemIndicator ;
	rdfs:label "UrbanPlanningIndicator"@en ;
	rdfs:comment "A set of indicators that is classified under Livelihood Support System, and contains various indicators under clause 21 from ISO 37120:2018, ISO 37122:2019 and ISO 37123:2019. For indicators stated in ISO 37120:2018, there are 3 further types of indicators - core, supporting and profile. Further details of these types of indicators are located at clause 3.4 of ISO 37120:2018."@en ;
	sh:targetClass indicators:UrbanPlanningIndicator ;
	.

indicators:WastewaterIndicator
	a
		owl:Class ,
		sh:NodeShape
		;
	rdfs:subClassOf indicators:EssentialServiceSystemIndicator ;
	rdfs:label "WastewaterIndicator"@en ;
	rdfs:comment "A set of indicators that is classified under Essential Service System, and contains various indicators under clause 22 from ISO 37120:2018, ISO 37122:2019 and ISO 37123:2019. For indicators stated in ISO 37120:2018, there are 3 further types of indicators - core, supporting and profile. Further details of these types of indicators are located at clause 3.4 of ISO 37120:2018."@en ;
	sh:targetClass indicators:WastewaterIndicator ;
	.

indicators:WaterIndicator
	a
		owl:Class ,
		sh:NodeShape
		;
	rdfs:subClassOf indicators:ResourceSystemIndicator ;
	rdfs:label "WaterIndicator"@en ;
	rdfs:comment "A set of indicators that is classified under Resource System, and contains various indicators under clause 23 from ISO 37120:2018, ISO 37122:2019 and ISO 37123:2019. For indicators stated in ISO 37120:2018, there are 3 further types of indicators - core, supporting and profile. Further details of these types of indicators are located at clause 3.4 of ISO 37120:2018."@en ;
	sh:targetClass indicators:WaterIndicator ;
	.